tests/refcore/Benchmark/Overview.hs
@@ -31,6 +31,12 @@ llen Nil = 0
 get :: IList -> Int -> Int
 get (Cons x xs') i' = if i' == 0 then x else get xs' (i' - 1)
 
+{-@ reflect evil @-}
+{-@ evil :: xs:IList -> x:{v:Int | 5 < v} -> i:{i:Int | 0 <= i } -> {get (Cons x xs) (i + 1) = get xs i } @-}
+evil :: IList -> Int -> Int -> Proof
+evil (Cons y ys) x i = if i == 0 then trivial else evil ys x (i-1)
+evil Nil x i = trivial
+
 -- Theorem
 
 {-@ thm1 :: xs:IList -> x:{v:Int | 5 < v} -> i:{i:Int | 0 <= i && i < (llen xs) }
