lava/out/Benchmark/PeanoNats.v
@@ -76,16 +76,16 @@ Defined.
 
 #[global] Hint Unfold Zero: ref_constr_db.
 
-Definition add_spec (ds_d4mE n : Nats): Type :=
+Definition add_spec (ds_d4oi n : Nats): Type :=
   Nats.
 
 #[global] Hint Unfold add_spec: lia_unfold.
 
-Definition add (ds_d4mE n : Nats): add_spec ds_d4mE n.
+Definition add (ds_d4oi n : Nats): add_spec ds_d4oi n.
 Proof.
-  destruct ds_d4mE as [ds_d4mE ds_d4mE_p].
+  destruct ds_d4oi as [ds_d4oi ds_d4oi_p].
   destruct n as [n n_p].
-  try revert n_p; generalize dependent n; induction ds_d4mE as [m IH_m|]; intros.
+  try revert n_p; generalize dependent n; induction ds_d4oi as [m IH_m|]; intros.
   - refine (Suc (IH_m ltac:(try clear IH_m; solver) n ltac:(try clear IH_m; solver))).
   - refine (exist (λ (n : Nats_u), Nats_wf n ∧ True) n ltac:(solver)).
 Defined.
@@ -100,10 +100,10 @@ Inductive add_rel: Nats_u → Nats_u → Nats_u → Prop :=
 
 #[global] Instance add_getF: getFunc add_rel := { getF' := add }.
 
-Theorem add_rel_funct [ds_d4mE n : Nats_u]:
-  ∀ (VV VV' : Nats_u), add_rel ds_d4mE n VV → (add_rel ds_d4mE n VV' → VV = VV').
+Theorem add_rel_funct [ds_d4oi n : Nats_u]:
+  ∀ (VV VV' : Nats_u), add_rel ds_d4oi n VV → (add_rel ds_d4oi n VV' → VV = VV').
 Proof.
-  try revert n_p; generalize dependent n; induction ds_d4mE as [m IH_m|]; intros;
+  try revert n_p; generalize dependent n; induction ds_d4oi as [m IH_m|]; intros;
   rel_functionhood_body.
 Qed.
 
@@ -129,12 +129,12 @@ Qed.
 #[global] Hint Rewrite add_Zero_x_lem: f_rel_back.
 
 Theorem add_rel_ex
-  (ds_d4mE : Nats_u) (ds_d4mE_p : Nats_wf ds_d4mE ∧ True) (n : Nats_u) (n_p : Nats_wf n ∧ True):
-  add_rel ds_d4mE n ⌊ add (exist _ ds_d4mE ds_d4mE_p) (exist _ n n_p) -⌋.
+  (ds_d4oi : Nats_u) (ds_d4oi_p : Nats_wf ds_d4oi ∧ True) (n : Nats_u) (n_p : Nats_wf n ∧ True):
+  add_rel ds_d4oi n ⌊ add (exist _ ds_d4oi ds_d4oi_p) (exist _ n n_p) -⌋.
 Proof.
   Opaque add.
   existence_lemma_pre add;
-  try revert n_p; generalize dependent n; induction ds_d4mE as [m IH_m|]; intros;
+  try revert n_p; generalize dependent n; induction ds_d4oi as [m IH_m|]; intros;
   [fix_notations;
    pose proof (IH_m ltac:(try clear IH_m; solver) n ltac:(try clear IH_m; solver)) as IH_14792487;
    try clear IH_m |
@@ -149,12 +149,12 @@ Qed.
 #[global] Opaque add.
 
 Theorem add__add_rel_rw
-  (ds_d4mE : Nats_u)
-  (ds_d4mE_p : Nats_wf ds_d4mE ∧ True)
+  (ds_d4oi : Nats_u)
+  (ds_d4oi_p : Nats_wf ds_d4oi ∧ True)
   (n : Nats_u)
   (n_p : Nats_wf n ∧ True)
   (VV : Nats_u):
-  ⌊ add (exist _ ds_d4mE ds_d4mE_p) (exist _ n n_p) -⌋ = VV ↔ add_rel ds_d4mE n VV.
+  ⌊ add (exist _ ds_d4oi ds_d4oi_p) (exist _ n n_p) -⌋ = VV ↔ add_rel ds_d4oi n VV.
 Proof.
   f__f_rel_rw.
 Qed.
@@ -165,31 +165,31 @@ Qed.
 
 #[global] Instance add_lookup_rw: dictionary rwLem add := { lookup' := add__add_rel_rw }.
 
-Theorem add__add_rel (ds_d4mE n : Nats) (VV : Nats_u):
-  ⌊ add ds_d4mE n -⌋ = VV ↔ add_rel ⌊ ds_d4mE ⌋ ⌊ n ⌋ VV.
+Theorem add__add_rel (ds_d4oi n : Nats) (VV : Nats_u):
+  ⌊ add ds_d4oi n -⌋ = VV ↔ add_rel ⌊ ds_d4oi ⌋ ⌊ n ⌋ VV.
 Proof.
   f__f_rel.
 Qed.
 
 #[global] Hint Rewrite add__add_rel: f_rel_funct_db.
 
-Theorem add__add_rel' (ds_d4mE_u n_u : Nats_u) (ds_d4mE n : Nats) (VV : Nats_u):
-  ds_d4mE_u = ⌊ ds_d4mE ⌋ → (n_u = ⌊ n ⌋ → ⌊ add ds_d4mE n -⌋ = VV ↔ add_rel ds_d4mE_u n_u VV).
+Theorem add__add_rel' (ds_d4oi_u n_u : Nats_u) (ds_d4oi n : Nats) (VV : Nats_u):
+  ds_d4oi_u = ⌊ ds_d4oi ⌋ → (n_u = ⌊ n ⌋ → ⌊ add ds_d4oi n -⌋ = VV ↔ add_rel ds_d4oi_u n_u VV).
 Proof.
-  intros -> ->. refine (add__add_rel ds_d4mE n VV).
+  intros -> ->. refine (add__add_rel ds_d4oi n VV).
 Qed.
 
 #[global] Hint Resolve add__add_rel': f_rel_funct_db.
 
 Theorem add_rel_mk
-  (ds_d4mE : Nats_u) (ds_d4mE_p : Nats_wf ds_d4mE ∧ True) (n : Nats_u) (n_p : Nats_wf n ∧ True):
-  {VV: _ | add_rel ds_d4mE n VV}.
+  (ds_d4oi : Nats_u) (ds_d4oi_p : Nats_wf ds_d4oi ∧ True) (n : Nats_u) (n_p : Nats_wf n ∧ True):
+  {VV: _ | add_rel ds_d4oi n VV}.
 Proof.
   intros;
   refine (subsumptionCast
           _
-          (λ VV, add_rel ds_d4mE n VV)
-          (add (exist _ ds_d4mE ds_d4mE_p) (exist _ n n_p))
+          (λ VV, add_rel ds_d4oi n VV)
+          (add (exist _ ds_d4oi ds_d4oi_p) (exist _ n n_p))
           _);
   rewrite <- add__add_rel';
   quicksolve.
@@ -199,13 +199,13 @@ Qed.
 
 #[global] Instance add_pack:
   @Pack
-  (Nats ::RT λ (ds_d4mE : Nats), Nats ::RT λ (n : Nats), nilRT)
+  (Nats ::RT λ (ds_d4oi : Nats), Nats ::RT λ (n : Nats), nilRT)
   (Nats_u ::UT (Nats_u ::UT nilUT))
-  ltac:(mkProjectsArgListTG (Nats ::RT λ (ds_d4mE : Nats), Nats ::RT λ (n : Nats), nilRT) ((Nats_u ::UT (Nats_u ::UT nilUT))))
+  ltac:(mkProjectsArgListTG (Nats ::RT λ (ds_d4oi : Nats), Nats ::RT λ (n : Nats), nilRT) ((Nats_u ::UT (Nats_u ::UT nilUT))))
   Nats_u
-  (λ (x_44855413 : ArgList (Nats ::RT λ (ds_d4mE : Nats), Nats ::RT λ (n : Nats), nilRT))
-     (v_x_44855413 : Nats_u),
-   ltac:(flattenP (λ (ds_d4mE n : Nats) (VV : Nats_u), Nats_wf VV ∧ True) x_44855413 v_x_44855413)).
+  (λ (x_65232642 : ArgList (Nats ::RT λ (ds_d4oi : Nats), Nats ::RT λ (n : Nats), nilRT))
+     (v_x_65232642 : Nats_u),
+   ltac:(flattenP (λ (ds_d4oi n : Nats) (VV : Nats_u), Nats_wf VV ∧ True) x_65232642 v_x_65232642)).
 Proof.
   buildPackG add add_rel add__add_rel add_rel_funct.
 Defined.
@@ -259,97 +259,97 @@ Proof.
           ltac:(solver)).
 Defined.
 
-Definition add_assoc_spec (ds_d4my ds_d4mz ds_d4mA : Nats): Type :=
+Definition add_assoc_spec (ds_d4oc ds_d4od ds_d4oe : Nats): Type :=
   {{∃ (add_res : Nats_u),
-    add_rel ⌊ ds_d4mz -⌋ ⌊ ds_d4mA -⌋ add_res
+    add_rel ⌊ ds_d4od -⌋ ⌊ ds_d4oe -⌋ add_res
     ∧ ∃ (add_res_2 : Nats_u),
-      add_rel ⌊ ds_d4my -⌋ add_res add_res_2
+      add_rel ⌊ ds_d4oc -⌋ add_res add_res_2
       ∧ ∃ (add_res_3 : Nats_u),
-        add_rel ⌊ ds_d4my -⌋ ⌊ ds_d4mz -⌋ add_res_3
-        ∧ ∃ (add_res_4 : Nats_u), add_rel add_res_3 ⌊ ds_d4mA -⌋ add_res_4 ∧ add_res_2 == add_res_4}}.
+        add_rel ⌊ ds_d4oc -⌋ ⌊ ds_d4od -⌋ add_res_3
+        ∧ ∃ (add_res_4 : Nats_u), add_rel add_res_3 ⌊ ds_d4oe -⌋ add_res_4 ∧ add_res_2 == add_res_4}}.
 
 #[global] Hint Unfold add_assoc_spec: lia_unfold.
 
-Theorem add_assoc (ds_d4my ds_d4mz ds_d4mA : Nats): add_assoc_spec ds_d4my ds_d4mz ds_d4mA.
+Theorem add_assoc (ds_d4oc ds_d4od ds_d4oe : Nats): add_assoc_spec ds_d4oc ds_d4od ds_d4oe.
 Proof.
-  destruct ds_d4my as [ds_d4my ds_d4my_p].
-  destruct ds_d4mz as [ds_d4mz ds_d4mz_p].
-  destruct ds_d4mA as [ds_d4mA ds_d4mA_p].
-  try revert ds_d4mA_p; generalize dependent ds_d4mA;
-  try revert ds_d4mz_p; generalize dependent ds_d4mz;
-  induction ds_d4my as [m IH_m|];
+  destruct ds_d4oc as [ds_d4oc ds_d4oc_p].
+  destruct ds_d4od as [ds_d4od ds_d4od_p].
+  destruct ds_d4oe as [ds_d4oe ds_d4oe_p].
+  try revert ds_d4oe_p; generalize dependent ds_d4oe;
+  try revert ds_d4od_p; generalize dependent ds_d4od;
+  induction ds_d4oc as [m IH_m|];
   intros.
   - refine (subsumptionCast
             Unit
             (λ (VV : Unit),
              ∃ (add_res : Nats_u),
-             add_rel ds_d4mz ds_d4mA add_res
+             add_rel ds_d4od ds_d4oe add_res
              ∧ ∃ (add_res_2 : Nats_u),
                add_rel (Suc_u m) add_res add_res_2
                ∧ ∃ (add_res_3 : Nats_u),
-                 add_rel (Suc_u m) ds_d4mz add_res_3
-                 ∧ ∃ (add_res_4 : Nats_u), add_rel add_res_3 ds_d4mA add_res_4 ∧ add_res_2 == add_res_4)
+                 add_rel (Suc_u m) ds_d4od add_res_3
+                 ∧ ∃ (add_res_4 : Nats_u), add_rel add_res_3 ds_d4oe add_res_4 ∧ add_res_2 == add_res_4)
             (IH_m
              ltac:(try clear IH_m; solver)
-             ds_d4mz
+             ds_d4od
              ltac:(try clear IH_m; solver)
-             ds_d4mA
+             ds_d4oe
              ltac:(try clear IH_m; solver))
             ltac:(solver)).
   - refine (subsumptionCast
             Unit
             (λ (VV : Unit),
              ∃ (add_res : Nats_u),
-             add_rel ds_d4mz ds_d4mA add_res
+             add_rel ds_d4od ds_d4oe add_res
              ∧ ∃ (add_res_2 : Nats_u),
                add_rel Zero_u add_res add_res_2
                ∧ ∃ (add_res_3 : Nats_u),
-                 add_rel Zero_u ds_d4mz add_res_3
-                 ∧ ∃ (add_res_4 : Nats_u), add_rel add_res_3 ds_d4mA add_res_4 ∧ add_res_2 == add_res_4)
+                 add_rel Zero_u ds_d4od add_res_3
+                 ∧ ∃ (add_res_4 : Nats_u), add_rel add_res_3 ds_d4oe add_res_4 ∧ add_res_2 == add_res_4)
             (# unit)
             ltac:(solver)).
 Qed.
 
-Definition add_suc_r_spec (ds_d4mn ds_d4mo : Nats): Type :=
+Definition add_suc_r_spec (ds_d4o1 ds_d4o2 : Nats): Type :=
   {{∃ (add_res : Nats_u),
-    add_rel ⌊ ds_d4mn -⌋ ⌊ ds_d4mo -⌋ add_res
+    add_rel ⌊ ds_d4o1 -⌋ ⌊ ds_d4o2 -⌋ add_res
     ∧ ∃ (add_res_2 : Nats_u),
-      add_rel ⌊ ds_d4mn -⌋ (Suc_u ⌊ ds_d4mo -⌋) add_res_2 ∧ Suc_u add_res == add_res_2}}.
+      add_rel ⌊ ds_d4o1 -⌋ (Suc_u ⌊ ds_d4o2 -⌋) add_res_2 ∧ Suc_u add_res == add_res_2}}.
 
 #[global] Hint Unfold add_suc_r_spec: lia_unfold.
 
-Theorem add_suc_r (ds_d4mn ds_d4mo : Nats): add_suc_r_spec ds_d4mn ds_d4mo.
+Theorem add_suc_r (ds_d4o1 ds_d4o2 : Nats): add_suc_r_spec ds_d4o1 ds_d4o2.
 Proof.
-  destruct ds_d4mn as [ds_d4mn ds_d4mn_p].
-  destruct ds_d4mo as [ds_d4mo ds_d4mo_p].
-  try revert ds_d4mo_p; generalize dependent ds_d4mo; induction ds_d4mn as [m IH_m|]; intros.
+  destruct ds_d4o1 as [ds_d4o1 ds_d4o1_p].
+  destruct ds_d4o2 as [ds_d4o2 ds_d4o2_p].
+  try revert ds_d4o2_p; generalize dependent ds_d4o2; induction ds_d4o1 as [m IH_m|]; intros.
   - refine (subsumptionCast
             Unit
             (λ (VV : Unit),
              ∃ (add_res : Nats_u),
-             add_rel (Suc_u m) ds_d4mo add_res
-             ∧ ∃ (add_res_2 : Nats_u), add_rel (Suc_u m) (Suc_u ds_d4mo) add_res_2 ∧ Suc_u add_res == add_res_2)
-            (IH_m ltac:(try clear IH_m; solver) ds_d4mo ltac:(try clear IH_m; solver))
+             add_rel (Suc_u m) ds_d4o2 add_res
+             ∧ ∃ (add_res_2 : Nats_u), add_rel (Suc_u m) (Suc_u ds_d4o2) add_res_2 ∧ Suc_u add_res == add_res_2)
+            (IH_m ltac:(try clear IH_m; solver) ds_d4o2 ltac:(try clear IH_m; solver))
             ltac:(solver)).
   - refine (subsumptionCast
             Unit
             (λ (VV : Unit),
              ∃ (add_res : Nats_u),
-             add_rel Zero_u ds_d4mo add_res
-             ∧ ∃ (add_res_2 : Nats_u), add_rel Zero_u (Suc_u ds_d4mo) add_res_2 ∧ Suc_u add_res == add_res_2)
+             add_rel Zero_u ds_d4o2 add_res
+             ∧ ∃ (add_res_2 : Nats_u), add_rel Zero_u (Suc_u ds_d4o2) add_res_2 ∧ Suc_u add_res == add_res_2)
             (# unit)
             ltac:(solver)).
 Qed.
 
-Definition add_zero_l_spec (ds_d4mB : Nats): Type :=
-  {{∃ (add_res : Nats_u), add_rel Zero_u ⌊ ds_d4mB -⌋ add_res ∧ add_res == ⌊ ds_d4mB -⌋}}.
+Definition add_zero_l_spec (ds_d4of : Nats): Type :=
+  {{∃ (add_res : Nats_u), add_rel Zero_u ⌊ ds_d4of -⌋ add_res ∧ add_res == ⌊ ds_d4of -⌋}}.
 
 #[global] Hint Unfold add_zero_l_spec: lia_unfold.
 
-Theorem add_zero_l (ds_d4mB : Nats): add_zero_l_spec ds_d4mB.
+Theorem add_zero_l (ds_d4of : Nats): add_zero_l_spec ds_d4of.
 Proof.
-  destruct ds_d4mB as [ds_d4mB ds_d4mB_p].
-  induction ds_d4mB as [n IH_n|].
+  destruct ds_d4of as [ds_d4of ds_d4of_p].
+  induction ds_d4of as [n IH_n|].
   - refine (subsumptionCast
             Unit
             (λ (VV : Unit), ∃ (add_res : Nats_u), add_rel Zero_u (Suc_u n) add_res ∧ add_res == Suc_u n)
@@ -379,15 +379,15 @@ Proof.
           ltac:(solver)).
 Qed.
 
-Definition add_zero_r_spec (ds_d4mp : Nats): Type :=
-  {{∃ (add_res : Nats_u), add_rel ⌊ ds_d4mp -⌋ Zero_u add_res ∧ add_res == ⌊ ds_d4mp -⌋}}.
+Definition add_zero_r_spec (ds_d4o3 : Nats): Type :=
+  {{∃ (add_res : Nats_u), add_rel ⌊ ds_d4o3 -⌋ Zero_u add_res ∧ add_res == ⌊ ds_d4o3 -⌋}}.
 
 #[global] Hint Unfold add_zero_r_spec: lia_unfold.
 
-Theorem add_zero_r (ds_d4mp : Nats): add_zero_r_spec ds_d4mp.
+Theorem add_zero_r (ds_d4o3 : Nats): add_zero_r_spec ds_d4o3.
 Proof.
-  destruct ds_d4mp as [ds_d4mp ds_d4mp_p].
-  induction ds_d4mp as [n IH_n|].
+  destruct ds_d4o3 as [ds_d4o3 ds_d4o3_p].
+  induction ds_d4o3 as [n IH_n|].
   - refine (subsumptionCast
             Unit
             (λ (VV : Unit), ∃ (add_res : Nats_u), add_rel (Suc_u n) Zero_u add_res ∧ add_res == Suc_u n)
@@ -400,20 +400,20 @@ Proof.
             ltac:(solver)).
 Qed.
 
-Definition eqN_spec (ds_d4m1 ds_d4m2 : Nats): Type :=
+Definition eqN_spec (ds_d4nF ds_d4nG : Nats): Type :=
   Bool.
 
 #[global] Hint Unfold eqN_spec: lia_unfold.
 
-Definition eqN (ds_d4m1 ds_d4m2 : Nats): eqN_spec ds_d4m1 ds_d4m2.
+Definition eqN (ds_d4nF ds_d4nG : Nats): eqN_spec ds_d4nF ds_d4nG.
 Proof.
-  destruct ds_d4m1 as [ds_d4m1 ds_d4m1_p].
-  destruct ds_d4m2 as [ds_d4m2 ds_d4m2_p].
-  try revert ds_d4m2_p; generalize dependent ds_d4m2; induction ds_d4m1 as [m IH_m|]; intros.
-  - destruct ds_d4m2 as [n|].
+  destruct ds_d4nF as [ds_d4nF ds_d4nF_p].
+  destruct ds_d4nG as [ds_d4nG ds_d4nG_p].
+  try revert ds_d4nG_p; generalize dependent ds_d4nG; induction ds_d4nF as [m IH_m|]; intros.
+  - destruct ds_d4nG as [n|].
     + refine (IH_m ltac:(try clear IH_m; solver) n ltac:(try clear IH_m; solver)).
     + refine (# false).
-  - destruct ds_d4m2 as [lq_anf7205759403792810464|].
+  - destruct ds_d4nG as [lq_anf7205759403792810566|].
     + refine (# false).
     + refine (# true).
 Defined.
@@ -421,7 +421,7 @@ Defined.
 Inductive eqN_rel: Nats_u → Nats_u → bool → Prop :=
   | eqN_Suc_Suc: ∀ m n (eqN_res : bool), eqN_rel m n eqN_res → eqN_rel (Suc_u m) (Suc_u n) eqN_res
   | eqN_Suc_Zero: ∀ m, eqN_rel (Suc_u m) Zero_u false
-  | eqN_Zero_Suc: ∀ lq_anf7205759403792810464, eqN_rel Zero_u (Suc_u lq_anf7205759403792810464) false
+  | eqN_Zero_Suc: ∀ lq_anf7205759403792810566, eqN_rel Zero_u (Suc_u lq_anf7205759403792810566) false
   | eqN_Zero_Zero: eqN_rel Zero_u Zero_u true.
 
 #[global] Hint Constructors eqN_rel: core_hint_db.
@@ -430,11 +430,11 @@ Inductive eqN_rel: Nats_u → Nats_u → bool → Prop :=
 
 #[global] Instance eqN_getF: getFunc eqN_rel := { getF' := eqN }.
 
-Theorem eqN_rel_funct [ds_d4m1 ds_d4m2 : Nats_u]:
-  ∀ (VV VV' : bool), eqN_rel ds_d4m1 ds_d4m2 VV → (eqN_rel ds_d4m1 ds_d4m2 VV' → VV = VV').
+Theorem eqN_rel_funct [ds_d4nF ds_d4nG : Nats_u]:
+  ∀ (VV VV' : bool), eqN_rel ds_d4nF ds_d4nG VV → (eqN_rel ds_d4nF ds_d4nG VV' → VV = VV').
 Proof.
-  try revert ds_d4m2_p; generalize dependent ds_d4m2; induction ds_d4m1 as [m IH_m|]; intros;
-  [destruct ds_d4m2 as [n|] | destruct ds_d4m2 as [lq_anf7205759403792810464|]];
+  try revert ds_d4nG_p; generalize dependent ds_d4nG; induction ds_d4nF as [m IH_m|]; intros;
+  [destruct ds_d4nG as [n|] | destruct ds_d4nG as [lq_anf7205759403792810566|]];
   rel_functionhood_body.
 Qed.
 
@@ -459,8 +459,8 @@ Qed.
 
 #[global] Hint Rewrite eqN_Suc_Zero_lem: f_rel_back.
 
-Theorem eqN_Zero_Suc_lem lq_anf7205759403792810464 eqN_Zero_Suc_lem_res:
-  eqN_rel Zero_u (Suc_u lq_anf7205759403792810464) eqN_Zero_Suc_lem_res
+Theorem eqN_Zero_Suc_lem lq_anf7205759403792810566 eqN_Zero_Suc_lem_res:
+  eqN_rel Zero_u (Suc_u lq_anf7205759403792810566) eqN_Zero_Suc_lem_res
   ↔ eqN_Zero_Suc_lem_res == false.
 Proof.
   rel_back' _nil.
@@ -477,21 +477,21 @@ Qed.
 #[global] Hint Rewrite eqN_Zero_Zero_lem: f_rel_back.
 
 Theorem eqN_rel_ex
-  (ds_d4m1 : Nats_u)
-  (ds_d4m1_p : Nats_wf ds_d4m1 ∧ True)
-  (ds_d4m2 : Nats_u)
-  (ds_d4m2_p : Nats_wf ds_d4m2 ∧ True):
-  eqN_rel ds_d4m1 ds_d4m2 ⌊ eqN (exist _ ds_d4m1 ds_d4m1_p) (exist _ ds_d4m2 ds_d4m2_p) -⌋.
+  (ds_d4nF : Nats_u)
+  (ds_d4nF_p : Nats_wf ds_d4nF ∧ True)
+  (ds_d4nG : Nats_u)
+  (ds_d4nG_p : Nats_wf ds_d4nG ∧ True):
+  eqN_rel ds_d4nF ds_d4nG ⌊ eqN (exist _ ds_d4nF ds_d4nF_p) (exist _ ds_d4nG ds_d4nG_p) -⌋.
 Proof.
   Opaque eqN.
   existence_lemma_pre eqN;
-  try revert ds_d4m2_p; generalize dependent ds_d4m2; induction ds_d4m1 as [m IH_m|]; intros;
-  [destruct ds_d4m2 as [n|];
+  try revert ds_d4nG_p; generalize dependent ds_d4nG; induction ds_d4nF as [m IH_m|]; intros;
+  [destruct ds_d4nG as [n|];
    [fix_notations;
     pose proof (IH_m ltac:(try clear IH_m; solver) n ltac:(try clear IH_m; solver)) as IH_14792487;
     try clear IH_m |
     fix_notations] |
-   destruct ds_d4m2 as [lq_anf7205759403792810464|];
+   destruct ds_d4nG as [lq_anf7205759403792810566|];
    [fix_notations | fix_notations]];
   simpl in *.
   Transparent eqN.
@@ -503,12 +503,12 @@ Qed.
 #[global] Opaque eqN.
 
 Theorem eqN__eqN_rel_rw
-  (ds_d4m1 : Nats_u)
-  (ds_d4m1_p : Nats_wf ds_d4m1 ∧ True)
-  (ds_d4m2 : Nats_u)
-  (ds_d4m2_p : Nats_wf ds_d4m2 ∧ True)
+  (ds_d4nF : Nats_u)
+  (ds_d4nF_p : Nats_wf ds_d4nF ∧ True)
+  (ds_d4nG : Nats_u)
+  (ds_d4nG_p : Nats_wf ds_d4nG ∧ True)
   (VV : bool):
-  ⌊ eqN (exist _ ds_d4m1 ds_d4m1_p) (exist _ ds_d4m2 ds_d4m2_p) -⌋ = VV ↔ eqN_rel ds_d4m1 ds_d4m2 VV.
+  ⌊ eqN (exist _ ds_d4nF ds_d4nF_p) (exist _ ds_d4nG ds_d4nG_p) -⌋ = VV ↔ eqN_rel ds_d4nF ds_d4nG VV.
 Proof.
   f__f_rel_rw.
 Qed.
@@ -519,35 +519,35 @@ Qed.
 
 #[global] Instance eqN_lookup_rw: dictionary rwLem eqN := { lookup' := eqN__eqN_rel_rw }.
 
-Theorem eqN__eqN_rel (ds_d4m1 ds_d4m2 : Nats) (VV : bool):
-  ⌊ eqN ds_d4m1 ds_d4m2 -⌋ = VV ↔ eqN_rel ⌊ ds_d4m1 ⌋ ⌊ ds_d4m2 ⌋ VV.
+Theorem eqN__eqN_rel (ds_d4nF ds_d4nG : Nats) (VV : bool):
+  ⌊ eqN ds_d4nF ds_d4nG -⌋ = VV ↔ eqN_rel ⌊ ds_d4nF ⌋ ⌊ ds_d4nG ⌋ VV.
 Proof.
   f__f_rel.
 Qed.
 
 #[global] Hint Rewrite eqN__eqN_rel: f_rel_funct_db.
 
-Theorem eqN__eqN_rel' (ds_d4m1_u ds_d4m2_u : Nats_u) (ds_d4m1 ds_d4m2 : Nats) (VV : bool):
-  ds_d4m1_u = ⌊ ds_d4m1 ⌋
-  → (ds_d4m2_u = ⌊ ds_d4m2 ⌋ → ⌊ eqN ds_d4m1 ds_d4m2 -⌋ = VV ↔ eqN_rel ds_d4m1_u ds_d4m2_u VV).
+Theorem eqN__eqN_rel' (ds_d4nF_u ds_d4nG_u : Nats_u) (ds_d4nF ds_d4nG : Nats) (VV : bool):
+  ds_d4nF_u = ⌊ ds_d4nF ⌋
+  → (ds_d4nG_u = ⌊ ds_d4nG ⌋ → ⌊ eqN ds_d4nF ds_d4nG -⌋ = VV ↔ eqN_rel ds_d4nF_u ds_d4nG_u VV).
 Proof.
-  intros -> ->. refine (eqN__eqN_rel ds_d4m1 ds_d4m2 VV).
+  intros -> ->. refine (eqN__eqN_rel ds_d4nF ds_d4nG VV).
 Qed.
 
 #[global] Hint Resolve eqN__eqN_rel': f_rel_funct_db.
 
 Theorem eqN_rel_mk
-  (ds_d4m1 : Nats_u)
-  (ds_d4m1_p : Nats_wf ds_d4m1 ∧ True)
-  (ds_d4m2 : Nats_u)
-  (ds_d4m2_p : Nats_wf ds_d4m2 ∧ True):
-  {VV: _ | eqN_rel ds_d4m1 ds_d4m2 VV}.
+  (ds_d4nF : Nats_u)
+  (ds_d4nF_p : Nats_wf ds_d4nF ∧ True)
+  (ds_d4nG : Nats_u)
+  (ds_d4nG_p : Nats_wf ds_d4nG ∧ True):
+  {VV: _ | eqN_rel ds_d4nF ds_d4nG VV}.
 Proof.
   intros;
   refine (subsumptionCast
           _
-          (λ VV, eqN_rel ds_d4m1 ds_d4m2 VV)
-          (eqN (exist _ ds_d4m1 ds_d4m1_p) (exist _ ds_d4m2 ds_d4m2_p))
+          (λ VV, eqN_rel ds_d4nF ds_d4nG VV)
+          (eqN (exist _ ds_d4nF ds_d4nF_p) (exist _ ds_d4nG ds_d4nG_p))
           _);
   rewrite <- eqN__eqN_rel';
   quicksolve.
@@ -557,13 +557,13 @@ Qed.
 
 #[global] Instance eqN_pack:
   @Pack
-  (Nats ::RT λ (ds_d4m1 : Nats), Nats ::RT λ (ds_d4m2 : Nats), nilRT)
+  (Nats ::RT λ (ds_d4nF : Nats), Nats ::RT λ (ds_d4nG : Nats), nilRT)
   (Nats_u ::UT (Nats_u ::UT nilUT))
-  ltac:(mkProjectsArgListTG (Nats ::RT λ (ds_d4m1 : Nats), Nats ::RT λ (ds_d4m2 : Nats), nilRT) ((Nats_u ::UT (Nats_u ::UT nilUT))))
+  ltac:(mkProjectsArgListTG (Nats ::RT λ (ds_d4nF : Nats), Nats ::RT λ (ds_d4nG : Nats), nilRT) ((Nats_u ::UT (Nats_u ::UT nilUT))))
   bool
-  (λ (x_41244053 : ArgList (Nats ::RT λ (ds_d4m1 : Nats), Nats ::RT λ (ds_d4m2 : Nats), nilRT))
-     (v_x_41244053 : bool),
-   ltac:(flattenP (λ (ds_d4m1 ds_d4m2 : Nats) (VV : bool), True) x_41244053 v_x_41244053)).
+  (λ (x_28156604 : ArgList (Nats ::RT λ (ds_d4nF : Nats), Nats ::RT λ (ds_d4nG : Nats), nilRT))
+     (v_x_28156604 : bool),
+   ltac:(flattenP (λ (ds_d4nF ds_d4nG : Nats) (VV : bool), True) x_28156604 v_x_28156604)).
 Proof.
   buildPackG eqN eqN_rel eqN__eqN_rel eqN_rel_funct.
 Defined.
@@ -601,34 +601,34 @@ Proof.
           ltac:(solver)).
 Defined.
 
-Definition geqN_spec (ds_d4mg ds_d4mh : Nats): Type :=
+Definition geqN_spec (ds_d4nU ds_d4nV : Nats): Type :=
   Bool.
 
 #[global] Hint Unfold geqN_spec: lia_unfold.
 
-Definition geqN (ds_d4mg ds_d4mh : Nats): geqN_spec ds_d4mg ds_d4mh.
+Definition geqN (ds_d4nU ds_d4nV : Nats): geqN_spec ds_d4nU ds_d4nV.
 Proof.
-  destruct ds_d4mg as [ds_d4mg ds_d4mg_p].
-  destruct ds_d4mh as [ds_d4mh ds_d4mh_p].
-  try revert ds_d4mg_p; generalize dependent ds_d4mg;
-  induction ds_d4mh as [lq_anf7205759403792810461 IH_lq_anf7205759403792810461|];
+  destruct ds_d4nU as [ds_d4nU ds_d4nU_p].
+  destruct ds_d4nV as [ds_d4nV ds_d4nV_p].
+  try revert ds_d4nU_p; generalize dependent ds_d4nU;
+  induction ds_d4nV as [lq_anf7205759403792810563 IH_lq_anf7205759403792810563|];
   intros.
-  - destruct ds_d4mg as [m|].
-    + refine (IH_lq_anf7205759403792810461
-              ltac:(try clear IH_lq_anf7205759403792810461; solver)
+  - destruct ds_d4nU as [m|].
+    + refine (IH_lq_anf7205759403792810563
+              ltac:(try clear IH_lq_anf7205759403792810563; solver)
               m
-              ltac:(try clear IH_lq_anf7205759403792810461; solver)).
+              ltac:(try clear IH_lq_anf7205759403792810563; solver)).
     + refine (# false).
   - refine (# true).
 Defined.
 
 Inductive geqN_rel: Nats_u → Nats_u → bool → Prop :=
-  | geqN_Suc_Suc: ∀ m lq_anf7205759403792810461 (geqN_res : bool),
-                  geqN_rel m lq_anf7205759403792810461 geqN_res
-                  → geqN_rel (Suc_u m) (Suc_u lq_anf7205759403792810461) geqN_res
-  | geqN_Zero_Suc: ∀ lq_anf7205759403792810461,
-                   geqN_rel Zero_u (Suc_u lq_anf7205759403792810461) false
-  | geqN_x_Zero: ∀ ds_d4mg, geqN_rel ds_d4mg Zero_u true.
+  | geqN_Suc_Suc: ∀ m lq_anf7205759403792810563 (geqN_res : bool),
+                  geqN_rel m lq_anf7205759403792810563 geqN_res
+                  → geqN_rel (Suc_u m) (Suc_u lq_anf7205759403792810563) geqN_res
+  | geqN_Zero_Suc: ∀ lq_anf7205759403792810563,
+                   geqN_rel Zero_u (Suc_u lq_anf7205759403792810563) false
+  | geqN_x_Zero: ∀ ds_d4nU, geqN_rel ds_d4nU Zero_u true.
 
 #[global] Hint Constructors geqN_rel: core_hint_db.
 
@@ -636,13 +636,13 @@ Inductive geqN_rel: Nats_u → Nats_u → bool → Prop :=
 
 #[global] Instance geqN_getF: getFunc geqN_rel := { getF' := geqN }.
 
-Theorem geqN_rel_funct [ds_d4mg ds_d4mh : Nats_u]:
-  ∀ (VV VV' : bool), geqN_rel ds_d4mg ds_d4mh VV → (geqN_rel ds_d4mg ds_d4mh VV' → VV = VV').
+Theorem geqN_rel_funct [ds_d4nU ds_d4nV : Nats_u]:
+  ∀ (VV VV' : bool), geqN_rel ds_d4nU ds_d4nV VV → (geqN_rel ds_d4nU ds_d4nV VV' → VV = VV').
 Proof.
-  try revert ds_d4mg_p; generalize dependent ds_d4mg;
-  induction ds_d4mh as [lq_anf7205759403792810461 IH_lq_anf7205759403792810461|];
+  try revert ds_d4nU_p; generalize dependent ds_d4nU;
+  induction ds_d4nV as [lq_anf7205759403792810563 IH_lq_anf7205759403792810563|];
   intros;
-  [destruct ds_d4mg as [m|] |];
+  [destruct ds_d4nU as [m|] |];
   rel_functionhood_body.
 Qed.
 
@@ -651,18 +651,18 @@ Qed.
 #[global] Instance geqN_lookup_funct: dictionary functionhood geqN := {
     lookup' := geqN_rel_funct }.
 
-Theorem geqN_Suc_Suc_lem lq_anf7205759403792810461 m geqN_Suc_Suc_lem_res:
-  geqN_rel (Suc_u m) (Suc_u lq_anf7205759403792810461) geqN_Suc_Suc_lem_res
+Theorem geqN_Suc_Suc_lem lq_anf7205759403792810563 m geqN_Suc_Suc_lem_res:
+  geqN_rel (Suc_u m) (Suc_u lq_anf7205759403792810563) geqN_Suc_Suc_lem_res
   ↔ ∃ (geqN_res : bool),
-    geqN_rel m lq_anf7205759403792810461 geqN_res ∧ geqN_Suc_Suc_lem_res == geqN_res.
+    geqN_rel m lq_anf7205759403792810563 geqN_res ∧ geqN_Suc_Suc_lem_res == geqN_res.
 Proof.
   rel_back' _nil.
 Qed.
 
 #[global] Hint Rewrite geqN_Suc_Suc_lem: f_rel_back.
 
-Theorem geqN_Zero_Suc_lem lq_anf7205759403792810461 geqN_Zero_Suc_lem_res:
-  geqN_rel Zero_u (Suc_u lq_anf7205759403792810461) geqN_Zero_Suc_lem_res
+Theorem geqN_Zero_Suc_lem lq_anf7205759403792810563 geqN_Zero_Suc_lem_res:
+  geqN_rel Zero_u (Suc_u lq_anf7205759403792810563) geqN_Zero_Suc_lem_res
   ↔ geqN_Zero_Suc_lem_res == false.
 Proof.
   rel_back' _nil.
@@ -670,8 +670,8 @@ Qed.
 
 #[global] Hint Rewrite geqN_Zero_Suc_lem: f_rel_back.
 
-Theorem geqN_x_Zero_lem ds_d4mg geqN_x_Zero_lem_res:
-  geqN_rel ds_d4mg Zero_u geqN_x_Zero_lem_res ↔ geqN_x_Zero_lem_res == true.
+Theorem geqN_x_Zero_lem ds_d4nU geqN_x_Zero_lem_res:
+  geqN_rel ds_d4nU Zero_u geqN_x_Zero_lem_res ↔ geqN_x_Zero_lem_res == true.
 Proof.
   rel_back' _nil.
 Qed.
@@ -679,24 +679,24 @@ Qed.
 #[global] Hint Rewrite geqN_x_Zero_lem: f_rel_back.
 
 Theorem geqN_rel_ex
-  (ds_d4mg : Nats_u)
-  (ds_d4mg_p : Nats_wf ds_d4mg ∧ True)
-  (ds_d4mh : Nats_u)
-  (ds_d4mh_p : Nats_wf ds_d4mh ∧ True):
-  geqN_rel ds_d4mg ds_d4mh ⌊ geqN (exist _ ds_d4mg ds_d4mg_p) (exist _ ds_d4mh ds_d4mh_p) -⌋.
+  (ds_d4nU : Nats_u)
+  (ds_d4nU_p : Nats_wf ds_d4nU ∧ True)
+  (ds_d4nV : Nats_u)
+  (ds_d4nV_p : Nats_wf ds_d4nV ∧ True):
+  geqN_rel ds_d4nU ds_d4nV ⌊ geqN (exist _ ds_d4nU ds_d4nU_p) (exist _ ds_d4nV ds_d4nV_p) -⌋.
 Proof.
   Opaque geqN.
   existence_lemma_pre geqN;
-  try revert ds_d4mg_p; generalize dependent ds_d4mg;
-  induction ds_d4mh as [lq_anf7205759403792810461 IH_lq_anf7205759403792810461|];
+  try revert ds_d4nU_p; generalize dependent ds_d4nU;
+  induction ds_d4nV as [lq_anf7205759403792810563 IH_lq_anf7205759403792810563|];
   intros;
-  [destruct ds_d4mg as [m|];
+  [destruct ds_d4nU as [m|];
    [fix_notations;
-    pose proof (IH_lq_anf7205759403792810461
-                ltac:(try clear IH_lq_anf7205759403792810461; solver)
+    pose proof (IH_lq_anf7205759403792810563
+                ltac:(try clear IH_lq_anf7205759403792810563; solver)
                 m
-                ltac:(try clear IH_lq_anf7205759403792810461; solver)) as IH_28387485;
-    try clear IH_lq_anf7205759403792810461 |
+                ltac:(try clear IH_lq_anf7205759403792810563; solver)) as IH_55853897;
+    try clear IH_lq_anf7205759403792810563 |
     fix_notations] |
    fix_notations];
   simpl in *.
@@ -709,13 +709,13 @@ Qed.
 #[global] Opaque geqN.
 
 Theorem geqN__geqN_rel_rw
-  (ds_d4mg : Nats_u)
-  (ds_d4mg_p : Nats_wf ds_d4mg ∧ True)
-  (ds_d4mh : Nats_u)
-  (ds_d4mh_p : Nats_wf ds_d4mh ∧ True)
+  (ds_d4nU : Nats_u)
+  (ds_d4nU_p : Nats_wf ds_d4nU ∧ True)
+  (ds_d4nV : Nats_u)
+  (ds_d4nV_p : Nats_wf ds_d4nV ∧ True)
   (VV : bool):
-  ⌊ geqN (exist _ ds_d4mg ds_d4mg_p) (exist _ ds_d4mh ds_d4mh_p) -⌋ = VV
-  ↔ geqN_rel ds_d4mg ds_d4mh VV.
+  ⌊ geqN (exist _ ds_d4nU ds_d4nU_p) (exist _ ds_d4nV ds_d4nV_p) -⌋ = VV
+  ↔ geqN_rel ds_d4nU ds_d4nV VV.
 Proof.
   f__f_rel_rw.
 Qed.
@@ -726,35 +726,35 @@ Qed.
 
 #[global] Instance geqN_lookup_rw: dictionary rwLem geqN := { lookup' := geqN__geqN_rel_rw }.
 
-Theorem geqN__geqN_rel (ds_d4mg ds_d4mh : Nats) (VV : bool):
-  ⌊ geqN ds_d4mg ds_d4mh -⌋ = VV ↔ geqN_rel ⌊ ds_d4mg ⌋ ⌊ ds_d4mh ⌋ VV.
+Theorem geqN__geqN_rel (ds_d4nU ds_d4nV : Nats) (VV : bool):
+  ⌊ geqN ds_d4nU ds_d4nV -⌋ = VV ↔ geqN_rel ⌊ ds_d4nU ⌋ ⌊ ds_d4nV ⌋ VV.
 Proof.
   f__f_rel.
 Qed.
 
 #[global] Hint Rewrite geqN__geqN_rel: f_rel_funct_db.
 
-Theorem geqN__geqN_rel' (ds_d4mg_u ds_d4mh_u : Nats_u) (ds_d4mg ds_d4mh : Nats) (VV : bool):
-  ds_d4mg_u = ⌊ ds_d4mg ⌋
-  → (ds_d4mh_u = ⌊ ds_d4mh ⌋ → ⌊ geqN ds_d4mg ds_d4mh -⌋ = VV ↔ geqN_rel ds_d4mg_u ds_d4mh_u VV).
+Theorem geqN__geqN_rel' (ds_d4nU_u ds_d4nV_u : Nats_u) (ds_d4nU ds_d4nV : Nats) (VV : bool):
+  ds_d4nU_u = ⌊ ds_d4nU ⌋
+  → (ds_d4nV_u = ⌊ ds_d4nV ⌋ → ⌊ geqN ds_d4nU ds_d4nV -⌋ = VV ↔ geqN_rel ds_d4nU_u ds_d4nV_u VV).
 Proof.
-  intros -> ->. refine (geqN__geqN_rel ds_d4mg ds_d4mh VV).
+  intros -> ->. refine (geqN__geqN_rel ds_d4nU ds_d4nV VV).
 Qed.
 
 #[global] Hint Resolve geqN__geqN_rel': f_rel_funct_db.
 
 Theorem geqN_rel_mk
-  (ds_d4mg : Nats_u)
-  (ds_d4mg_p : Nats_wf ds_d4mg ∧ True)
-  (ds_d4mh : Nats_u)
-  (ds_d4mh_p : Nats_wf ds_d4mh ∧ True):
-  {VV: _ | geqN_rel ds_d4mg ds_d4mh VV}.
+  (ds_d4nU : Nats_u)
+  (ds_d4nU_p : Nats_wf ds_d4nU ∧ True)
+  (ds_d4nV : Nats_u)
+  (ds_d4nV_p : Nats_wf ds_d4nV ∧ True):
+  {VV: _ | geqN_rel ds_d4nU ds_d4nV VV}.
 Proof.
   intros;
   refine (subsumptionCast
           _
-          (λ VV, geqN_rel ds_d4mg ds_d4mh VV)
-          (geqN (exist _ ds_d4mg ds_d4mg_p) (exist _ ds_d4mh ds_d4mh_p))
+          (λ VV, geqN_rel ds_d4nU ds_d4nV VV)
+          (geqN (exist _ ds_d4nU ds_d4nU_p) (exist _ ds_d4nV ds_d4nV_p))
           _);
   rewrite <- geqN__geqN_rel';
   quicksolve.
@@ -764,13 +764,13 @@ Qed.
 
 #[global] Instance geqN_pack:
   @Pack
-  (Nats ::RT λ (ds_d4mg : Nats), Nats ::RT λ (ds_d4mh : Nats), nilRT)
+  (Nats ::RT λ (ds_d4nU : Nats), Nats ::RT λ (ds_d4nV : Nats), nilRT)
   (Nats_u ::UT (Nats_u ::UT nilUT))
-  ltac:(mkProjectsArgListTG (Nats ::RT λ (ds_d4mg : Nats), Nats ::RT λ (ds_d4mh : Nats), nilRT) ((Nats_u ::UT (Nats_u ::UT nilUT))))
+  ltac:(mkProjectsArgListTG (Nats ::RT λ (ds_d4nU : Nats), Nats ::RT λ (ds_d4nV : Nats), nilRT) ((Nats_u ::UT (Nats_u ::UT nilUT))))
   bool
-  (λ (x_35960879 : ArgList (Nats ::RT λ (ds_d4mg : Nats), Nats ::RT λ (ds_d4mh : Nats), nilRT))
-     (v_x_35960879 : bool),
-   ltac:(flattenP (λ (ds_d4mg ds_d4mh : Nats) (VV : bool), True) x_35960879 v_x_35960879)).
+  (λ (x_13635317 : ArgList (Nats ::RT λ (ds_d4nU : Nats), Nats ::RT λ (ds_d4nV : Nats), nilRT))
+     (v_x_13635317 : bool),
+   ltac:(flattenP (λ (ds_d4nU ds_d4nV : Nats) (VV : bool), True) x_13635317 v_x_13635317)).
 Proof.
   buildPackG geqN geqN_rel geqN__geqN_rel geqN_rel_funct.
 Defined.
@@ -780,27 +780,27 @@ Proof.
   buildUPackG geqN_rel geqN_rel_funct.
 Defined.
 
-Definition mult_spec (ds_d4mG ds_d4mH : Nats): Type :=
+Definition mult_spec (ds_d4ok ds_d4ol : Nats): Type :=
   Nats.
 
 #[global] Hint Unfold mult_spec: lia_unfold.
 
-Definition mult (ds_d4mG ds_d4mH : Nats): mult_spec ds_d4mG ds_d4mH.
+Definition mult (ds_d4ok ds_d4ol : Nats): mult_spec ds_d4ok ds_d4ol.
 Proof.
-  destruct ds_d4mG as [ds_d4mG ds_d4mG_p].
-  destruct ds_d4mH as [ds_d4mH ds_d4mH_p].
-  try revert ds_d4mH_p; generalize dependent ds_d4mH; induction ds_d4mG as [m IH_m|]; intros.
+  destruct ds_d4ok as [ds_d4ok ds_d4ok_p].
+  destruct ds_d4ol as [ds_d4ol ds_d4ol_p].
+  try revert ds_d4ol_p; generalize dependent ds_d4ol; induction ds_d4ok as [m IH_m|]; intros.
   - refine (add
-            (exist (λ (ds_d4mH : Nats_u), Nats_wf ds_d4mH ∧ True) ds_d4mH ltac:(solver))
-            (IH_m ltac:(try clear IH_m; solver) ds_d4mH ltac:(try clear IH_m; solver))).
+            (exist (λ (ds_d4ol : Nats_u), Nats_wf ds_d4ol ∧ True) ds_d4ol ltac:(solver))
+            (IH_m ltac:(try clear IH_m; solver) ds_d4ol ltac:(try clear IH_m; solver))).
   - refine Zero.
 Defined.
 
 Inductive mult_rel: Nats_u → Nats_u → Nats_u → Prop :=
-  | mult_Suc_x: ∀ m ds_d4mH (mult_res : Nats_u),
-                mult_rel m ds_d4mH mult_res
-                → ∀ (add_res : Nats_u), add_rel ds_d4mH mult_res add_res → mult_rel (Suc_u m) ds_d4mH add_res
-  | mult_Zero_x: ∀ ds_d4mH, mult_rel Zero_u ds_d4mH Zero_u.
+  | mult_Suc_x: ∀ m ds_d4ol (mult_res : Nats_u),
+                mult_rel m ds_d4ol mult_res
+                → ∀ (add_res : Nats_u), add_rel ds_d4ol mult_res add_res → mult_rel (Suc_u m) ds_d4ol add_res
+  | mult_Zero_x: ∀ ds_d4ol, mult_rel Zero_u ds_d4ol Zero_u.
 
 #[global] Hint Constructors mult_rel: core_hint_db.
 
@@ -808,10 +808,10 @@ Inductive mult_rel: Nats_u → Nats_u → Nats_u → Prop :=
 
 #[global] Instance mult_getF: getFunc mult_rel := { getF' := mult }.
 
-Theorem mult_rel_funct [ds_d4mG ds_d4mH : Nats_u]:
-  ∀ (VV VV' : Nats_u), mult_rel ds_d4mG ds_d4mH VV → (mult_rel ds_d4mG ds_d4mH VV' → VV = VV').
+Theorem mult_rel_funct [ds_d4ok ds_d4ol : Nats_u]:
+  ∀ (VV VV' : Nats_u), mult_rel ds_d4ok ds_d4ol VV → (mult_rel ds_d4ok ds_d4ol VV' → VV = VV').
 Proof.
-  try revert ds_d4mH_p; generalize dependent ds_d4mH; induction ds_d4mG as [m IH_m|]; intros;
+  try revert ds_d4ol_p; generalize dependent ds_d4ol; induction ds_d4ok as [m IH_m|]; intros;
   rel_functionhood_body.
 Qed.
 
@@ -820,19 +820,19 @@ Qed.
 #[global] Instance mult_lookup_funct: dictionary functionhood mult := {
     lookup' := mult_rel_funct }.
 
-Theorem mult_Suc_x_lem ds_d4mH m mult_Suc_x_lem_res:
-  mult_rel (Suc_u m) ds_d4mH mult_Suc_x_lem_res
+Theorem mult_Suc_x_lem ds_d4ol m mult_Suc_x_lem_res:
+  mult_rel (Suc_u m) ds_d4ol mult_Suc_x_lem_res
   ↔ ∃ (mult_res : Nats_u),
-    mult_rel m ds_d4mH mult_res
-    ∧ ∃ (add_res : Nats_u), add_rel ds_d4mH mult_res add_res ∧ mult_Suc_x_lem_res == add_res.
+    mult_rel m ds_d4ol mult_res
+    ∧ ∃ (add_res : Nats_u), add_rel ds_d4ol mult_res add_res ∧ mult_Suc_x_lem_res == add_res.
 Proof.
   rel_back' _nil.
 Qed.
 
 #[global] Hint Rewrite mult_Suc_x_lem: f_rel_back.
 
-Theorem mult_Zero_x_lem ds_d4mH mult_Zero_x_lem_res:
-  mult_rel Zero_u ds_d4mH mult_Zero_x_lem_res ↔ mult_Zero_x_lem_res == Zero_u.
+Theorem mult_Zero_x_lem ds_d4ol mult_Zero_x_lem_res:
+  mult_rel Zero_u ds_d4ol mult_Zero_x_lem_res ↔ mult_Zero_x_lem_res == Zero_u.
 Proof.
   rel_back' _nil.
 Qed.
@@ -840,20 +840,20 @@ Qed.
 #[global] Hint Rewrite mult_Zero_x_lem: f_rel_back.
 
 Theorem mult_rel_ex
-  (ds_d4mG : Nats_u)
-  (ds_d4mG_p : Nats_wf ds_d4mG ∧ True)
-  (ds_d4mH : Nats_u)
-  (ds_d4mH_p : Nats_wf ds_d4mH ∧ True):
-  mult_rel ds_d4mG ds_d4mH ⌊ mult (exist _ ds_d4mG ds_d4mG_p) (exist _ ds_d4mH ds_d4mH_p) -⌋.
+  (ds_d4ok : Nats_u)
+  (ds_d4ok_p : Nats_wf ds_d4ok ∧ True)
+  (ds_d4ol : Nats_u)
+  (ds_d4ol_p : Nats_wf ds_d4ol ∧ True):
+  mult_rel ds_d4ok ds_d4ol ⌊ mult (exist _ ds_d4ok ds_d4ok_p) (exist _ ds_d4ol ds_d4ol_p) -⌋.
 Proof.
   Opaque mult.
   existence_lemma_pre mult;
-  try revert ds_d4mH_p; generalize dependent ds_d4mH; induction ds_d4mG as [m IH_m|]; intros;
+  try revert ds_d4ol_p; generalize dependent ds_d4ol; induction ds_d4ok as [m IH_m|]; intros;
   [fix_notations;
    pose proof (IH_m
                ltac:(try clear IH_m; solver)
-               ds_d4mH
-               ltac:(try clear IH_m; solver)) as IH_74478145;
+               ds_d4ol
+               ltac:(try clear IH_m; solver)) as IH_89830954;
    try clear IH_m |
    fix_notations];
   simpl in *.
@@ -866,13 +866,13 @@ Qed.
 #[global] Opaque mult.
 
 Theorem mult__mult_rel_rw
-  (ds_d4mG : Nats_u)
-  (ds_d4mG_p : Nats_wf ds_d4mG ∧ True)
-  (ds_d4mH : Nats_u)
-  (ds_d4mH_p : Nats_wf ds_d4mH ∧ True)
+  (ds_d4ok : Nats_u)
+  (ds_d4ok_p : Nats_wf ds_d4ok ∧ True)
+  (ds_d4ol : Nats_u)
+  (ds_d4ol_p : Nats_wf ds_d4ol ∧ True)
   (VV : Nats_u):
-  ⌊ mult (exist _ ds_d4mG ds_d4mG_p) (exist _ ds_d4mH ds_d4mH_p) -⌋ = VV
-  ↔ mult_rel ds_d4mG ds_d4mH VV.
+  ⌊ mult (exist _ ds_d4ok ds_d4ok_p) (exist _ ds_d4ol ds_d4ol_p) -⌋ = VV
+  ↔ mult_rel ds_d4ok ds_d4ol VV.
 Proof.
   f__f_rel_rw.
 Qed.
@@ -883,35 +883,35 @@ Qed.
 
 #[global] Instance mult_lookup_rw: dictionary rwLem mult := { lookup' := mult__mult_rel_rw }.
 
-Theorem mult__mult_rel (ds_d4mG ds_d4mH : Nats) (VV : Nats_u):
-  ⌊ mult ds_d4mG ds_d4mH -⌋ = VV ↔ mult_rel ⌊ ds_d4mG ⌋ ⌊ ds_d4mH ⌋ VV.
+Theorem mult__mult_rel (ds_d4ok ds_d4ol : Nats) (VV : Nats_u):
+  ⌊ mult ds_d4ok ds_d4ol -⌋ = VV ↔ mult_rel ⌊ ds_d4ok ⌋ ⌊ ds_d4ol ⌋ VV.
 Proof.
   f__f_rel.
 Qed.
 
 #[global] Hint Rewrite mult__mult_rel: f_rel_funct_db.
 
-Theorem mult__mult_rel' (ds_d4mG_u ds_d4mH_u : Nats_u) (ds_d4mG ds_d4mH : Nats) (VV : Nats_u):
-  ds_d4mG_u = ⌊ ds_d4mG ⌋
-  → (ds_d4mH_u = ⌊ ds_d4mH ⌋ → ⌊ mult ds_d4mG ds_d4mH -⌋ = VV ↔ mult_rel ds_d4mG_u ds_d4mH_u VV).
+Theorem mult__mult_rel' (ds_d4ok_u ds_d4ol_u : Nats_u) (ds_d4ok ds_d4ol : Nats) (VV : Nats_u):
+  ds_d4ok_u = ⌊ ds_d4ok ⌋
+  → (ds_d4ol_u = ⌊ ds_d4ol ⌋ → ⌊ mult ds_d4ok ds_d4ol -⌋ = VV ↔ mult_rel ds_d4ok_u ds_d4ol_u VV).
 Proof.
-  intros -> ->. refine (mult__mult_rel ds_d4mG ds_d4mH VV).
+  intros -> ->. refine (mult__mult_rel ds_d4ok ds_d4ol VV).
 Qed.
 
 #[global] Hint Resolve mult__mult_rel': f_rel_funct_db.
 
 Theorem mult_rel_mk
-  (ds_d4mG : Nats_u)
-  (ds_d4mG_p : Nats_wf ds_d4mG ∧ True)
-  (ds_d4mH : Nats_u)
-  (ds_d4mH_p : Nats_wf ds_d4mH ∧ True):
-  {VV: _ | mult_rel ds_d4mG ds_d4mH VV}.
+  (ds_d4ok : Nats_u)
+  (ds_d4ok_p : Nats_wf ds_d4ok ∧ True)
+  (ds_d4ol : Nats_u)
+  (ds_d4ol_p : Nats_wf ds_d4ol ∧ True):
+  {VV: _ | mult_rel ds_d4ok ds_d4ol VV}.
 Proof.
   intros;
   refine (subsumptionCast
           _
-          (λ VV, mult_rel ds_d4mG ds_d4mH VV)
-          (mult (exist _ ds_d4mG ds_d4mG_p) (exist _ ds_d4mH ds_d4mH_p))
+          (λ VV, mult_rel ds_d4ok ds_d4ol VV)
+          (mult (exist _ ds_d4ok ds_d4ok_p) (exist _ ds_d4ol ds_d4ol_p))
           _);
   rewrite <- mult__mult_rel';
   quicksolve.
@@ -921,13 +921,13 @@ Qed.
 
 #[global] Instance mult_pack:
   @Pack
-  (Nats ::RT λ (ds_d4mG : Nats), Nats ::RT λ (ds_d4mH : Nats), nilRT)
+  (Nats ::RT λ (ds_d4ok : Nats), Nats ::RT λ (ds_d4ol : Nats), nilRT)
   (Nats_u ::UT (Nats_u ::UT nilUT))
-  ltac:(mkProjectsArgListTG (Nats ::RT λ (ds_d4mG : Nats), Nats ::RT λ (ds_d4mH : Nats), nilRT) ((Nats_u ::UT (Nats_u ::UT nilUT))))
+  ltac:(mkProjectsArgListTG (Nats ::RT λ (ds_d4ok : Nats), Nats ::RT λ (ds_d4ol : Nats), nilRT) ((Nats_u ::UT (Nats_u ::UT nilUT))))
   Nats_u
-  (λ (x_75073885 : ArgList (Nats ::RT λ (ds_d4mG : Nats), Nats ::RT λ (ds_d4mH : Nats), nilRT))
-     (v_x_75073885 : Nats_u),
-   ltac:(flattenP (λ (ds_d4mG ds_d4mH : Nats) (VV : Nats_u), Nats_wf VV ∧ True) x_75073885 v_x_75073885)).
+  (λ (x_51015715 : ArgList (Nats ::RT λ (ds_d4ok : Nats), Nats ::RT λ (ds_d4ol : Nats), nilRT))
+     (v_x_51015715 : Nats_u),
+   ltac:(flattenP (λ (ds_d4ok ds_d4ol : Nats) (VV : Nats_u), Nats_wf VV ∧ True) x_51015715 v_x_51015715)).
 Proof.
   buildPackG mult mult_rel mult__mult_rel mult_rel_funct.
 Defined.
@@ -937,80 +937,85 @@ Proof.
   buildUPackG mult_rel mult_rel_funct.
 Defined.
 
-Definition add_dist_rmult_spec (ds_d4mI ds_d4mJ ds_d4mK : Nats): Type :=
+Definition add_dist_rmult_spec (ds_d4om ds_d4on ds_d4oo : Nats): Type :=
   {{∃ (add_res : Nats_u),
-    add_rel ⌊ ds_d4mI -⌋ ⌊ ds_d4mJ -⌋ add_res
+    add_rel ⌊ ds_d4om -⌋ ⌊ ds_d4on -⌋ add_res
     ∧ ∃ (mult_res : Nats_u),
-      mult_rel add_res ⌊ ds_d4mK -⌋ mult_res
+      mult_rel add_res ⌊ ds_d4oo -⌋ mult_res
       ∧ ∃ (mult_res_2 : Nats_u),
-        mult_rel ⌊ ds_d4mJ -⌋ ⌊ ds_d4mK -⌋ mult_res_2
+        mult_rel ⌊ ds_d4on -⌋ ⌊ ds_d4oo -⌋ mult_res_2
         ∧ ∃ (mult_res_3 : Nats_u),
-          mult_rel ⌊ ds_d4mI -⌋ ⌊ ds_d4mK -⌋ mult_res_3
+          mult_rel ⌊ ds_d4om -⌋ ⌊ ds_d4oo -⌋ mult_res_3
           ∧ ∃ (add_res_2 : Nats_u), add_rel mult_res_3 mult_res_2 add_res_2 ∧ mult_res == add_res_2}}.
 
 #[global] Hint Unfold add_dist_rmult_spec: lia_unfold.
 
-Theorem add_dist_rmult (ds_d4mI ds_d4mJ ds_d4mK : Nats):
-  add_dist_rmult_spec ds_d4mI ds_d4mJ ds_d4mK.
+Theorem add_dist_rmult (ds_d4om ds_d4on ds_d4oo : Nats):
+  add_dist_rmult_spec ds_d4om ds_d4on ds_d4oo.
 Proof.
-  destruct ds_d4mI as [ds_d4mI ds_d4mI_p].
-  destruct ds_d4mJ as [ds_d4mJ ds_d4mJ_p].
-  destruct ds_d4mK as [ds_d4mK ds_d4mK_p].
-  destruct ds_d4mI as [m|].
-  - assert (h_61850938 : add
-                         ds_d4mK
+  destruct ds_d4om as [ds_d4om ds_d4om_p].
+  destruct ds_d4on as [ds_d4on ds_d4on_p].
+  destruct ds_d4oo as [ds_d4oo ds_d4oo_p].
+  try revert ds_d4oo_p; generalize dependent ds_d4oo;
+  try revert ds_d4on_p; generalize dependent ds_d4on;
+  induction ds_d4om as [m IH_m|];
+  intros.
+  - assert (h_78908773 : add
+                         ds_d4oo
                          (add
                           ⌊ mult
                             (exist (λ (n : Nats_u), Nats_wf n ∧ True) m ltac:(solver))
-                            (exist (λ (ds_d4mK : Nats_u), Nats_wf ds_d4mK ∧ True) ds_d4mK ltac:(solver)) -⌋
+                            (exist (λ (ds_d4oo : Nats_u), Nats_wf ds_d4oo ∧ True) ds_d4oo ltac:(solver)) -⌋
                           ⌊ mult
-                            (exist (λ (ds_d4mJ : Nats_u), Nats_wf ds_d4mJ ∧ True) ds_d4mJ ltac:(solver))
-                            (exist (λ (ds_d4mK : Nats_u), Nats_wf ds_d4mK ∧ True) ds_d4mK ltac:(solver)) -⌋)
+                            (exist (λ (ds_d4on : Nats_u), Nats_wf ds_d4on ∧ True) ds_d4on ltac:(solver))
+                            (exist (λ (ds_d4oo : Nats_u), Nats_wf ds_d4oo ∧ True) ds_d4oo ltac:(solver)) -⌋)
                          ==? add
                              (add
-                              ds_d4mK
+                              ds_d4oo
                               ⌊ mult
                                 (exist (λ (n : Nats_u), Nats_wf n ∧ True) m ltac:(solver))
-                                (exist (λ (ds_d4mK : Nats_u), Nats_wf ds_d4mK ∧ True) ds_d4mK ltac:(solver)) -⌋)
+                                (exist (λ (ds_d4oo : Nats_u), Nats_wf ds_d4oo ∧ True) ds_d4oo ltac:(solver)) -⌋)
                              ⌊ mult
-                               (exist (λ (ds_d4mJ : Nats_u), Nats_wf ds_d4mJ ∧ True) ds_d4mJ ltac:(solver))
-                               (exist (λ (ds_d4mK : Nats_u), Nats_wf ds_d4mK ∧ True) ds_d4mK ltac:(solver)) -⌋).
+                               (exist (λ (ds_d4on : Nats_u), Nats_wf ds_d4on ∧ True) ds_d4on ltac:(solver))
+                               (exist (λ (ds_d4oo : Nats_u), Nats_wf ds_d4oo ∧ True) ds_d4oo ltac:(solver)) -⌋).
     { refine (add_assoc
-              (exist (λ (ds_d4mK : Nats_u), Nats_wf ds_d4mK ∧ True) ds_d4mK ltac:(solver))
+              (exist (λ (ds_d4oo : Nats_u), Nats_wf ds_d4oo ∧ True) ds_d4oo ltac:(solver))
               (mult
                (exist (λ (n : Nats_u), Nats_wf n ∧ True) m ltac:(solver))
-               (exist (λ (ds_d4mK : Nats_u), Nats_wf ds_d4mK ∧ True) ds_d4mK ltac:(solver)))
+               (exist (λ (ds_d4oo : Nats_u), Nats_wf ds_d4oo ∧ True) ds_d4oo ltac:(solver)))
               (mult
-               (exist (λ (ds_d4mJ : Nats_u), Nats_wf ds_d4mJ ∧ True) ds_d4mJ ltac:(solver))
-               (exist (λ (ds_d4mK : Nats_u), Nats_wf ds_d4mK ∧ True) ds_d4mK ltac:(solver)))). }
+               (exist (λ (ds_d4on : Nats_u), Nats_wf ds_d4on ∧ True) ds_d4on ltac:(solver))
+               (exist (λ (ds_d4oo : Nats_u), Nats_wf ds_d4oo ∧ True) ds_d4oo ltac:(solver)))). }
     refine (subsumptionCast
             Unit
             (λ (VV : Unit),
              ∃ (add_res : Nats_u),
-             add_rel (Suc_u m) ds_d4mJ add_res
+             add_rel (Suc_u m) ds_d4on add_res
              ∧ ∃ (mult_res : Nats_u),
-               mult_rel add_res ds_d4mK mult_res
+               mult_rel add_res ds_d4oo mult_res
                ∧ ∃ (mult_res_2 : Nats_u),
-                 mult_rel ds_d4mJ ds_d4mK mult_res_2
+                 mult_rel ds_d4on ds_d4oo mult_res_2
                  ∧ ∃ (mult_res_3 : Nats_u),
-                   mult_rel (Suc_u m) ds_d4mK mult_res_3
+                   mult_rel (Suc_u m) ds_d4oo mult_res_3
                    ∧ ∃ (add_res_2 : Nats_u), add_rel mult_res_3 mult_res_2 add_res_2 ∧ mult_res == add_res_2)
-            (add_dist_rmult
-             (exist (λ (n : Nats_u), Nats_wf n ∧ True) m ltac:(solver))
-             (exist (λ (ds_d4mJ : Nats_u), Nats_wf ds_d4mJ ∧ True) ds_d4mJ ltac:(solver))
-             (exist (λ (ds_d4mK : Nats_u), Nats_wf ds_d4mK ∧ True) ds_d4mK ltac:(solver)))
+            (IH_m
+             ltac:(try clear IH_m; solver)
+             ds_d4on
+             ltac:(try clear IH_m; solver)
+             ds_d4oo
+             ltac:(try clear IH_m; solver))
             ltac:(solver)).
   - refine (subsumptionCast
             Unit
             (λ (VV : Unit),
              ∃ (add_res : Nats_u),
-             add_rel Zero_u ds_d4mJ add_res
+             add_rel Zero_u ds_d4on add_res
              ∧ ∃ (mult_res : Nats_u),
-               mult_rel add_res ds_d4mK mult_res
+               mult_rel add_res ds_d4oo mult_res
                ∧ ∃ (mult_res_2 : Nats_u),
-                 mult_rel ds_d4mJ ds_d4mK mult_res_2
+                 mult_rel ds_d4on ds_d4oo mult_res_2
                  ∧ ∃ (mult_res_3 : Nats_u),
-                   mult_rel Zero_u ds_d4mK mult_res_3
+                   mult_rel Zero_u ds_d4oo mult_res_3
                    ∧ ∃ (add_res_2 : Nats_u), add_rel mult_res_3 mult_res_2 add_res_2 ∧ mult_res == add_res_2)
             (# unit)
             ltac:(solver)).
@@ -1027,24 +1032,24 @@ Proof.
 Defined.
 
 Definition sub_spec
-  (ds_d4lW : Nats)
-  (ds_d4lX : {ds_d4lX: Nats_u | Nats_wf ds_d4lX
-                                ∧ ∃ (geqN_res : bool), geqN_rel ⌊ ds_d4lW -⌋ ds_d4lX geqN_res ∧ is_true geqN_res}):
+  (ds_d4nA : Nats)
+  (ds_d4nB : {ds_d4nB: Nats_u | Nats_wf ds_d4nB
+                                ∧ ∃ (geqN_res : bool), geqN_rel ⌊ ds_d4nA -⌋ ds_d4nB geqN_res ∧ is_true geqN_res}):
   Type :=
-  {o: Nats_u | Nats_wf o ∧ (o ≠ Zero_u ↔ ⌊ ds_d4lW -⌋ ≠ ⌊ ds_d4lX -⌋)}.
+  {o: Nats_u | Nats_wf o ∧ (o ≠ Zero_u ↔ ⌊ ds_d4nA -⌋ ≠ ⌊ ds_d4nB -⌋)}.
 
 #[global] Hint Unfold sub_spec: lia_unfold.
 
 Definition sub
-  (ds_d4lW : Nats)
-  (ds_d4lX : {ds_d4lX: Nats_u | Nats_wf ds_d4lX
-                                ∧ ∃ (geqN_res : bool), geqN_rel ⌊ ds_d4lW -⌋ ds_d4lX geqN_res ∧ is_true geqN_res}):
-  sub_spec ds_d4lW ds_d4lX.
+  (ds_d4nA : Nats)
+  (ds_d4nB : {ds_d4nB: Nats_u | Nats_wf ds_d4nB
+                                ∧ ∃ (geqN_res : bool), geqN_rel ⌊ ds_d4nA -⌋ ds_d4nB geqN_res ∧ is_true geqN_res}):
+  sub_spec ds_d4nA ds_d4nB.
 Proof.
-  destruct ds_d4lW as [ds_d4lW ds_d4lW_p].
-  destruct ds_d4lX as [ds_d4lX ds_d4lX_p].
-  try revert ds_d4lX_p; generalize dependent ds_d4lX; induction ds_d4lW as [m IH_m|]; intros.
-  - destruct ds_d4lX as [n|].
+  destruct ds_d4nA as [ds_d4nA ds_d4nA_p].
+  destruct ds_d4nB as [ds_d4nB ds_d4nB_p].
+  try revert ds_d4nB_p; generalize dependent ds_d4nB; induction ds_d4nA as [m IH_m|]; intros.
+  - destruct ds_d4nB as [n|].
     + refine (subsumptionCast
               Nats_u
               (λ (o : Nats_u), Nats_wf o ∧ (o ≠ Zero_u ↔ Suc_u m ≠ Suc_u n))
@@ -1055,7 +1060,7 @@ Proof.
               (λ (o : Nats_u), Nats_wf o ∧ (o ≠ Zero_u ↔ Suc_u m ≠ Zero_u))
               (Suc (exist (λ (n : Nats_u), Nats_wf n ∧ True) m ltac:(solver)))
               ltac:(solver)).
-  - destruct ds_d4lX as [lq_anf7205759403792810480|].
+  - destruct ds_d4nB as [lq_anf7205759403792810582|].
     + intros; exfalso; solver.
     + refine (subsumptionCast
               Nats_u
@@ -1075,11 +1080,11 @@ Inductive sub_rel: Nats_u → Nats_u → Nats_u → Prop :=
 
 #[global] Instance sub_getF: getFunc sub_rel := { getF' := sub }.
 
-Theorem sub_rel_funct [ds_d4lW ds_d4lX : Nats_u]:
-  ∀ (o o' : Nats_u), sub_rel ds_d4lW ds_d4lX o → (sub_rel ds_d4lW ds_d4lX o' → o = o').
+Theorem sub_rel_funct [ds_d4nA ds_d4nB : Nats_u]:
+  ∀ (o o' : Nats_u), sub_rel ds_d4nA ds_d4nB o → (sub_rel ds_d4nA ds_d4nB o' → o = o').
 Proof.
-  try revert ds_d4lX_p; generalize dependent ds_d4lX; induction ds_d4lW as [m IH_m|]; intros;
-  [destruct ds_d4lX as [n|] | destruct ds_d4lX as [lq_anf7205759403792810480|]];
+  try revert ds_d4nB_p; generalize dependent ds_d4nB; induction ds_d4nA as [m IH_m|]; intros;
+  [destruct ds_d4nB as [n|] | destruct ds_d4nB as [lq_anf7205759403792810582|]];
   rel_functionhood_body.
 Qed.
 
@@ -1113,22 +1118,22 @@ Qed.
 #[global] Hint Rewrite sub_Zero_Zero_lem: f_rel_back.
 
 Theorem sub_rel_ex
-  (ds_d4lW : Nats_u)
-  (ds_d4lW_p : Nats_wf ds_d4lW ∧ True)
-  (ds_d4lX : Nats_u)
-  (ds_d4lX_p : Nats_wf ds_d4lX
-               ∧ ∃ (geqN_res : bool), geqN_rel ds_d4lW ds_d4lX geqN_res ∧ is_true geqN_res):
-  sub_rel ds_d4lW ds_d4lX ⌊ sub (exist _ ds_d4lW ds_d4lW_p) (exist _ ds_d4lX ds_d4lX_p) -⌋.
+  (ds_d4nA : Nats_u)
+  (ds_d4nA_p : Nats_wf ds_d4nA ∧ True)
+  (ds_d4nB : Nats_u)
+  (ds_d4nB_p : Nats_wf ds_d4nB
+               ∧ ∃ (geqN_res : bool), geqN_rel ds_d4nA ds_d4nB geqN_res ∧ is_true geqN_res):
+  sub_rel ds_d4nA ds_d4nB ⌊ sub (exist _ ds_d4nA ds_d4nA_p) (exist _ ds_d4nB ds_d4nB_p) -⌋.
 Proof.
   Opaque sub.
   existence_lemma_pre sub;
-  try revert ds_d4lX_p; generalize dependent ds_d4lX; induction ds_d4lW as [m IH_m|]; intros;
-  [destruct ds_d4lX as [n|];
+  try revert ds_d4nB_p; generalize dependent ds_d4nB; induction ds_d4nA as [m IH_m|]; intros;
+  [destruct ds_d4nB as [n|];
    [fix_notations;
     pose proof (IH_m ltac:(try clear IH_m; solver) n ltac:(try clear IH_m; solver)) as IH_14792487;
     try clear IH_m |
     fix_notations] |
-   destruct ds_d4lX as [lq_anf7205759403792810480|];
+   destruct ds_d4nB as [lq_anf7205759403792810582|];
    [ | fix_notations]];
   simpl in *.
   Transparent sub.
@@ -1140,13 +1145,13 @@ Qed.
 #[global] Opaque sub.
 
 Theorem sub__sub_rel_rw
-  (ds_d4lW : Nats_u)
-  (ds_d4lW_p : Nats_wf ds_d4lW ∧ True)
-  (ds_d4lX : Nats_u)
-  (ds_d4lX_p : Nats_wf ds_d4lX
-               ∧ ∃ (geqN_res : bool), geqN_rel ds_d4lW ds_d4lX geqN_res ∧ is_true geqN_res)
+  (ds_d4nA : Nats_u)
+  (ds_d4nA_p : Nats_wf ds_d4nA ∧ True)
+  (ds_d4nB : Nats_u)
+  (ds_d4nB_p : Nats_wf ds_d4nB
+               ∧ ∃ (geqN_res : bool), geqN_rel ds_d4nA ds_d4nB geqN_res ∧ is_true geqN_res)
   (o : Nats_u):
-  ⌊ sub (exist _ ds_d4lW ds_d4lW_p) (exist _ ds_d4lX ds_d4lX_p) -⌋ = o ↔ sub_rel ds_d4lW ds_d4lX o.
+  ⌊ sub (exist _ ds_d4nA ds_d4nA_p) (exist _ ds_d4nB ds_d4nB_p) -⌋ = o ↔ sub_rel ds_d4nA ds_d4nB o.
 Proof.
   f__f_rel_rw.
 Qed.
@@ -1158,11 +1163,11 @@ Qed.
 #[global] Instance sub_lookup_rw: dictionary rwLem sub := { lookup' := sub__sub_rel_rw }.
 
 Theorem sub__sub_rel
-  (ds_d4lW : Nats)
-  (ds_d4lX : {ds_d4lX: Nats_u | Nats_wf ds_d4lX
-                                ∧ ∃ (geqN_res : bool), geqN_rel ⌊ ds_d4lW -⌋ ds_d4lX geqN_res ∧ is_true geqN_res})
+  (ds_d4nA : Nats)
+  (ds_d4nB : {ds_d4nB: Nats_u | Nats_wf ds_d4nB
+                                ∧ ∃ (geqN_res : bool), geqN_rel ⌊ ds_d4nA -⌋ ds_d4nB geqN_res ∧ is_true geqN_res})
   (o : Nats_u):
-  ⌊ sub ds_d4lW ds_d4lX -⌋ = o ↔ sub_rel ⌊ ds_d4lW ⌋ ⌊ ds_d4lX ⌋ o.
+  ⌊ sub ds_d4nA ds_d4nB -⌋ = o ↔ sub_rel ⌊ ds_d4nA ⌋ ⌊ ds_d4nB ⌋ o.
 Proof.
   f__f_rel.
 Qed.
@@ -1170,32 +1175,32 @@ Qed.
 #[global] Hint Rewrite sub__sub_rel: f_rel_funct_db.
 
 Theorem sub__sub_rel'
-  (ds_d4lW_u ds_d4lX_u : Nats_u)
-  (ds_d4lW : Nats)
-  (ds_d4lX : {ds_d4lX: Nats_u | Nats_wf ds_d4lX
-                                ∧ ∃ (geqN_res : bool), geqN_rel ⌊ ds_d4lW -⌋ ds_d4lX geqN_res ∧ is_true geqN_res})
+  (ds_d4nA_u ds_d4nB_u : Nats_u)
+  (ds_d4nA : Nats)
+  (ds_d4nB : {ds_d4nB: Nats_u | Nats_wf ds_d4nB
+                                ∧ ∃ (geqN_res : bool), geqN_rel ⌊ ds_d4nA -⌋ ds_d4nB geqN_res ∧ is_true geqN_res})
   (o : Nats_u):
-  ds_d4lW_u = ⌊ ds_d4lW ⌋
-  → (ds_d4lX_u = ⌊ ds_d4lX ⌋ → ⌊ sub ds_d4lW ds_d4lX -⌋ = o ↔ sub_rel ds_d4lW_u ds_d4lX_u o).
+  ds_d4nA_u = ⌊ ds_d4nA ⌋
+  → (ds_d4nB_u = ⌊ ds_d4nB ⌋ → ⌊ sub ds_d4nA ds_d4nB -⌋ = o ↔ sub_rel ds_d4nA_u ds_d4nB_u o).
 Proof.
-  intros -> ->. refine (sub__sub_rel ds_d4lW ds_d4lX o).
+  intros -> ->. refine (sub__sub_rel ds_d4nA ds_d4nB o).
 Qed.
 
 #[global] Hint Resolve sub__sub_rel': f_rel_funct_db.
 
 Theorem sub_rel_mk
-  (ds_d4lW : Nats_u)
-  (ds_d4lW_p : Nats_wf ds_d4lW ∧ True)
-  (ds_d4lX : Nats_u)
-  (ds_d4lX_p : Nats_wf ds_d4lX
-               ∧ ∃ (geqN_res : bool), geqN_rel ds_d4lW ds_d4lX geqN_res ∧ is_true geqN_res):
-  {o: _ | sub_rel ds_d4lW ds_d4lX o}.
+  (ds_d4nA : Nats_u)
+  (ds_d4nA_p : Nats_wf ds_d4nA ∧ True)
+  (ds_d4nB : Nats_u)
+  (ds_d4nB_p : Nats_wf ds_d4nB
+               ∧ ∃ (geqN_res : bool), geqN_rel ds_d4nA ds_d4nB geqN_res ∧ is_true geqN_res):
+  {o: _ | sub_rel ds_d4nA ds_d4nB o}.
 Proof.
   intros;
   refine (subsumptionCast
           _
-          (λ o, sub_rel ds_d4lW ds_d4lX o)
-          (sub (exist _ ds_d4lW ds_d4lW_p) (exist _ ds_d4lX ds_d4lX_p))
+          (λ o, sub_rel ds_d4nA ds_d4nB o)
+          (sub (exist _ ds_d4nA ds_d4nA_p) (exist _ ds_d4nB ds_d4nB_p))
           _);
   rewrite <- sub__sub_rel';
   quicksolve.
@@ -1206,42 +1211,42 @@ Qed.
 #[global] Instance sub_pack:
   @Pack
   (Nats
-   ::RT λ (ds_d4lW : Nats),
-        {ds_d4lX: Nats_u | Nats_wf ds_d4lX
-                           ∧ ∃ (geqN_res : bool), geqN_rel ⌊ ds_d4lW -⌋ ds_d4lX geqN_res ∧ is_true geqN_res}
-        ::RT λ (ds_d4lX : {ds_d4lX: Nats_u | Nats_wf ds_d4lX
+   ::RT λ (ds_d4nA : Nats),
+        {ds_d4nB: Nats_u | Nats_wf ds_d4nB
+                           ∧ ∃ (geqN_res : bool), geqN_rel ⌊ ds_d4nA -⌋ ds_d4nB geqN_res ∧ is_true geqN_res}
+        ::RT λ (ds_d4nB : {ds_d4nB: Nats_u | Nats_wf ds_d4nB
                                              ∧ ∃ (geqN_res : bool),
-                                               geqN_rel ⌊ ds_d4lW -⌋ ds_d4lX geqN_res ∧ is_true geqN_res}),
+                                               geqN_rel ⌊ ds_d4nA -⌋ ds_d4nB geqN_res ∧ is_true geqN_res}),
              nilRT)
   (Nats_u ::UT (Nats_u ::UT nilUT))
   ltac:(mkProjectsArgListTG (Nats
- ::RT λ (ds_d4lW : Nats),
-      {ds_d4lX: Nats_u | Nats_wf ds_d4lX
+ ::RT λ (ds_d4nA : Nats),
+      {ds_d4nB: Nats_u | Nats_wf ds_d4nB
                          ∧ ∃ (geqN_res : bool),
-                           geqN_rel ⌊ ds_d4lW -⌋ ds_d4lX geqN_res ∧ is_true geqN_res}
-      ::RT λ (ds_d4lX : {ds_d4lX: Nats_u | Nats_wf ds_d4lX
+                           geqN_rel ⌊ ds_d4nA -⌋ ds_d4nB geqN_res ∧ is_true geqN_res}
+      ::RT λ (ds_d4nB : {ds_d4nB: Nats_u | Nats_wf ds_d4nB
                                            ∧ ∃ (geqN_res : bool),
-                                             geqN_rel ⌊ ds_d4lW -⌋ ds_d4lX geqN_res
+                                             geqN_rel ⌊ ds_d4nA -⌋ ds_d4nB geqN_res
                                              ∧ is_true geqN_res}),
            nilRT) ((Nats_u ::UT (Nats_u ::UT nilUT))))
   Nats_u
-  (λ (x_34844924 : ArgList (Nats
-                            ::RT λ (ds_d4lW : Nats),
-                                 {ds_d4lX: Nats_u | Nats_wf ds_d4lX
+  (λ (x_78071397 : ArgList (Nats
+                            ::RT λ (ds_d4nA : Nats),
+                                 {ds_d4nB: Nats_u | Nats_wf ds_d4nB
                                                     ∧ ∃ (geqN_res : bool),
-                                                      geqN_rel ⌊ ds_d4lW -⌋ ds_d4lX geqN_res ∧ is_true geqN_res}
-                                 ::RT λ (ds_d4lX : {ds_d4lX: Nats_u | Nats_wf ds_d4lX
+                                                      geqN_rel ⌊ ds_d4nA -⌋ ds_d4nB geqN_res ∧ is_true geqN_res}
+                                 ::RT λ (ds_d4nB : {ds_d4nB: Nats_u | Nats_wf ds_d4nB
                                                                       ∧ ∃ (geqN_res : bool),
-                                                                        geqN_rel ⌊ ds_d4lW -⌋ ds_d4lX geqN_res
+                                                                        geqN_rel ⌊ ds_d4nA -⌋ ds_d4nB geqN_res
                                                                         ∧ is_true geqN_res}),
                                       nilRT))
-     (v_x_34844924 : Nats_u),
-   ltac:(flattenP (λ (ds_d4lW : Nats)
-   (ds_d4lX : {ds_d4lX: Nats_u | Nats_wf ds_d4lX
+     (v_x_78071397 : Nats_u),
+   ltac:(flattenP (λ (ds_d4nA : Nats)
+   (ds_d4nB : {ds_d4nB: Nats_u | Nats_wf ds_d4nB
                                  ∧ ∃ (geqN_res : bool),
-                                   geqN_rel ⌊ ds_d4lW -⌋ ds_d4lX geqN_res ∧ is_true geqN_res})
+                                   geqN_rel ⌊ ds_d4nA -⌋ ds_d4nB geqN_res ∧ is_true geqN_res})
    (o : Nats_u),
- Nats_wf o ∧ (o ≠ Zero_u ↔ ⌊ ds_d4lW -⌋ ≠ ⌊ ds_d4lX -⌋)) x_34844924 v_x_34844924)).
+ Nats_wf o ∧ (o ≠ Zero_u ↔ ⌊ ds_d4nA -⌋ ≠ ⌊ ds_d4nB -⌋)) x_78071397 v_x_78071397)).
 Proof.
   buildPackG sub sub_rel sub__sub_rel sub_rel_funct.
 Defined.
@@ -1251,38 +1256,36 @@ Proof.
   buildUPackG sub_rel sub_rel_funct.
 Defined.
 
-Definition add_sub_spec (ds_d4mq ds_d4mr : Nats): Type :=
+Definition add_sub_spec (ds_d4o4 ds_d4o5 : Nats): Type :=
   {{∃ (add_res : Nats_u),
-    add_rel ⌊ ds_d4mq -⌋ ⌊ ds_d4mr -⌋ add_res
-    ∧ ∃ (sub_res : Nats_u), sub_rel add_res ⌊ ds_d4mr -⌋ sub_res ∧ sub_res == ⌊ ds_d4mq -⌋}}.
+    add_rel ⌊ ds_d4o4 -⌋ ⌊ ds_d4o5 -⌋ add_res
+    ∧ ∃ (sub_res : Nats_u), sub_rel add_res ⌊ ds_d4o5 -⌋ sub_res ∧ sub_res == ⌊ ds_d4o4 -⌋}}.
 
 #[global] Hint Unfold add_sub_spec: lia_unfold.
 
-Theorem add_sub (ds_d4mq ds_d4mr : Nats): add_sub_spec ds_d4mq ds_d4mr.
+Theorem add_sub (ds_d4o4 ds_d4o5 : Nats): add_sub_spec ds_d4o4 ds_d4o5.
 Proof.
-  destruct ds_d4mq as [ds_d4mq ds_d4mq_p].
-  destruct ds_d4mr as [ds_d4mr ds_d4mr_p].
-  destruct ds_d4mq as [m|].
-  - destruct ds_d4mr as [lq_anf7205759403792810450|].
-    + assert (h_65318599 : sub
+  destruct ds_d4o4 as [ds_d4o4 ds_d4o4_p].
+  destruct ds_d4o5 as [ds_d4o5 ds_d4o5_p].
+  destruct ds_d4o4 as [m|].
+  - induction ds_d4o5 as [lq_anf7205759403792810552 IH_lq_anf7205759403792810552|].
+    + assert (h_45011131 : sub
                            (add
                             ⌊ Suc (exist (λ (n : Nats_u), Nats_wf n ∧ True) m ltac:(solver)) -⌋
-                            lq_anf7205759403792810450)
-                           lq_anf7205759403792810450
+                            lq_anf7205759403792810552)
+                           lq_anf7205759403792810552
                            ==? ⌊ Suc (exist (λ (n : Nats_u), Nats_wf n ∧ True) m ltac:(solver)) -⌋).
-      { refine (add_sub
-                (Suc (exist (λ (n : Nats_u), Nats_wf n ∧ True) m ltac:(solver)))
-                (exist (λ (n : Nats_u), Nats_wf n ∧ True) lq_anf7205759403792810450 ltac:(solver))). }
+      { refine (IH_lq_anf7205759403792810552 ltac:(try clear IH_lq_anf7205759403792810552; solver)). }
       refine (subsumptionCast
               Unit
               (λ (VV : Unit),
                ∃ (add_res : Nats_u),
-               add_rel (Suc_u m) (Suc_u lq_anf7205759403792810450) add_res
+               add_rel (Suc_u m) (Suc_u lq_anf7205759403792810552) add_res
                ∧ ∃ (sub_res : Nats_u),
-                 sub_rel add_res (Suc_u lq_anf7205759403792810450) sub_res ∧ sub_res == Suc_u m)
+                 sub_rel add_res (Suc_u lq_anf7205759403792810552) sub_res ∧ sub_res == Suc_u m)
               (add_suc_r
                (Suc (exist (λ (n : Nats_u), Nats_wf n ∧ True) m ltac:(solver)))
-               (exist (λ (n : Nats_u), Nats_wf n ∧ True) lq_anf7205759403792810450 ltac:(solver)))
+               (exist (λ (n : Nats_u), Nats_wf n ∧ True) lq_anf7205759403792810552 ltac:(solver)))
               ltac:(solver)).
     + refine (subsumptionCast
               Unit
@@ -1292,20 +1295,18 @@ Proof.
                ∧ ∃ (sub_res : Nats_u), sub_rel add_res Zero_u sub_res ∧ sub_res == Suc_u m)
               (add_zero_r (exist (λ (n : Nats_u), Nats_wf n ∧ True) m ltac:(solver)))
               ltac:(solver)).
-  - destruct ds_d4mr as [lq_anf7205759403792810442|].
-    + assert (h_83124024 : sub (add ⌊ Zero -⌋ lq_anf7205759403792810442) lq_anf7205759403792810442
+  - induction ds_d4o5 as [lq_anf7205759403792810544 IH_lq_anf7205759403792810544|].
+    + assert (h_14964841 : sub (add ⌊ Zero -⌋ lq_anf7205759403792810544) lq_anf7205759403792810544
                            ==? ⌊ Zero -⌋).
-      { refine (add_sub
-                Zero
-                (exist (λ (n : Nats_u), Nats_wf n ∧ True) lq_anf7205759403792810442 ltac:(solver))). }
+      { refine (IH_lq_anf7205759403792810544 ltac:(try clear IH_lq_anf7205759403792810544; solver)). }
       refine (subsumptionCast
               Unit
               (λ (VV : Unit),
                ∃ (add_res : Nats_u),
-               add_rel Zero_u (Suc_u lq_anf7205759403792810442) add_res
+               add_rel Zero_u (Suc_u lq_anf7205759403792810544) add_res
                ∧ ∃ (sub_res : Nats_u),
-                 sub_rel add_res (Suc_u lq_anf7205759403792810442) sub_res ∧ sub_res == Zero_u)
-              (add_suc_r Zero (exist (λ (n : Nats_u), Nats_wf n ∧ True) lq_anf7205759403792810442 ltac:(solver)))
+                 sub_rel add_res (Suc_u lq_anf7205759403792810544) sub_res ∧ sub_res == Zero_u)
+              (add_suc_r Zero (exist (λ (n : Nats_u), Nats_wf n ∧ True) lq_anf7205759403792810544 ltac:(solver)))
               ltac:(solver)).
     + refine (subsumptionCast
               Unit
@@ -1317,18 +1318,18 @@ Proof.
               ltac:(solver)).
 Qed.
 
-Definition sub_self_spec (ds_d4lQ ds_d4lR : Nats): Type :=
-  {{∃ (eqN_res : bool), eqN_rel ⌊ ds_d4lQ -⌋ ⌊ ds_d4lR -⌋ eqN_res ∧ is_true eqN_res
-    → ∃ (sub_res : Nats_u), sub_rel ⌊ ds_d4lQ -⌋ ⌊ ds_d4lR -⌋ sub_res ∧ sub_res == Zero_u}}.
+Definition sub_self_spec (ds_d4nu ds_d4nv : Nats): Type :=
+  {{∃ (eqN_res : bool), eqN_rel ⌊ ds_d4nu -⌋ ⌊ ds_d4nv -⌋ eqN_res ∧ is_true eqN_res
+    → ∃ (sub_res : Nats_u), sub_rel ⌊ ds_d4nu -⌋ ⌊ ds_d4nv -⌋ sub_res ∧ sub_res == Zero_u}}.
 
 #[global] Hint Unfold sub_self_spec: lia_unfold.
 
-Theorem sub_self (ds_d4lQ ds_d4lR : Nats): sub_self_spec ds_d4lQ ds_d4lR.
+Theorem sub_self (ds_d4nu ds_d4nv : Nats): sub_self_spec ds_d4nu ds_d4nv.
 Proof.
-  destruct ds_d4lQ as [ds_d4lQ ds_d4lQ_p].
-  destruct ds_d4lR as [ds_d4lR ds_d4lR_p].
-  try revert ds_d4lR_p; generalize dependent ds_d4lR; induction ds_d4lQ as [m IH_m|]; intros.
-  - destruct ds_d4lR as [n|].
+  destruct ds_d4nu as [ds_d4nu ds_d4nu_p].
+  destruct ds_d4nv as [ds_d4nv ds_d4nv_p].
+  try revert ds_d4nv_p; generalize dependent ds_d4nv; induction ds_d4nu as [m IH_m|]; intros.
+  - destruct ds_d4nv as [n|].
     + refine (subsumptionCast
               Unit
               (λ (VV : Unit),
@@ -1346,8 +1347,8 @@ Proof.
   - refine (subsumptionCast
             Unit
             (λ (VV : Unit),
-             ∃ (eqN_res : bool), eqN_rel Zero_u ds_d4lR eqN_res ∧ is_true eqN_res
-             → ∃ (sub_res : Nats_u), sub_rel Zero_u ds_d4lR sub_res ∧ sub_res == Zero_u)
+             ∃ (eqN_res : bool), eqN_rel Zero_u ds_d4nv eqN_res ∧ is_true eqN_res
+             → ∃ (sub_res : Nats_u), sub_rel Zero_u ds_d4nv sub_res ∧ sub_res == Zero_u)
             (# unit)
             ltac:(solver)).
 Qed.
