lava/out/Benchmark/SoftwareFoundationsInduction.v
@@ -6,19 +6,19 @@ From Coq Require Import Unicode.Utf8.
 
 Load Benchmark.SoftwareFoundationsBasics.
 
-Definition plus_n_Sm_spec (ds_d9a8 m : MyNat): Type :=
+Definition plus_n_Sm_spec (ds_d9bM m : MyNat): Type :=
   {{∃ (plus_res : MyNat_u),
-    plus_rel ⌊ ds_d9a8 -⌋ ⌊ m -⌋ plus_res
+    plus_rel ⌊ ds_d9bM -⌋ ⌊ m -⌋ plus_res
     ∧ ∃ (plus_res_2 : MyNat_u),
-      plus_rel ⌊ ds_d9a8 -⌋ (S_u ⌊ m -⌋) plus_res_2 ∧ S_u plus_res == plus_res_2}}.
+      plus_rel ⌊ ds_d9bM -⌋ (S_u ⌊ m -⌋) plus_res_2 ∧ S_u plus_res == plus_res_2}}.
 
 #[global] Hint Unfold plus_n_Sm_spec: lia_unfold.
 
-Theorem plus_n_Sm (ds_d9a8 m : MyNat): plus_n_Sm_spec ds_d9a8 m.
+Theorem plus_n_Sm (ds_d9bM m : MyNat): plus_n_Sm_spec ds_d9bM m.
 Proof.
-  destruct ds_d9a8 as [ds_d9a8 ds_d9a8_p].
+  destruct ds_d9bM as [ds_d9bM ds_d9bM_p].
   destruct m as [m m_p].
-  try revert m_p; generalize dependent m; induction ds_d9a8 as [| n' IH_n']; intros.
+  try revert m_p; generalize dependent m; induction ds_d9bM as [| n' IH_n']; intros.
   - refine (subsumptionCast
             Unit
             (λ (VV : Unit),
@@ -37,15 +37,15 @@ Proof.
             ltac:(solver)).
 Qed.
 
-Definition mul_0_r_spec (ds_d9a9 : MyNat): Type :=
-  {{∃ (mult_res : MyNat_u), mult_rel ⌊ ds_d9a9 -⌋ O_u mult_res ∧ mult_res == O_u}}.
+Definition mul_0_r_spec (ds_d9bN : MyNat): Type :=
+  {{∃ (mult_res : MyNat_u), mult_rel ⌊ ds_d9bN -⌋ O_u mult_res ∧ mult_res == O_u}}.
 
 #[global] Hint Unfold mul_0_r_spec: lia_unfold.
 
-Theorem mul_0_r (ds_d9a9 : MyNat): mul_0_r_spec ds_d9a9.
+Theorem mul_0_r (ds_d9bN : MyNat): mul_0_r_spec ds_d9bN.
 Proof.
-  destruct ds_d9a9 as [ds_d9a9 ds_d9a9_p].
-  induction ds_d9a9 as [| n' IH_n'].
+  destruct ds_d9bN as [ds_d9bN ds_d9bN_p].
+  induction ds_d9bN as [| n' IH_n'].
   - refine (subsumptionCast
             Unit
             (λ (VV : Unit), ∃ (mult_res : MyNat_u), mult_rel O_u O_u mult_res ∧ mult_res == O_u)
@@ -58,15 +58,15 @@ Proof.
             ltac:(solver)).
 Qed.
 
-Definition minus_n_n_spec (ds_d9aa : MyNat): Type :=
-  {{∃ (minus_res : MyNat_u), minus_rel ⌊ ds_d9aa -⌋ ⌊ ds_d9aa -⌋ minus_res ∧ minus_res == O_u}}.
+Definition minus_n_n_spec (ds_d9bO : MyNat): Type :=
+  {{∃ (minus_res : MyNat_u), minus_rel ⌊ ds_d9bO -⌋ ⌊ ds_d9bO -⌋ minus_res ∧ minus_res == O_u}}.
 
 #[global] Hint Unfold minus_n_n_spec: lia_unfold.
 
-Theorem minus_n_n (ds_d9aa : MyNat): minus_n_n_spec ds_d9aa.
+Theorem minus_n_n (ds_d9bO : MyNat): minus_n_n_spec ds_d9bO.
 Proof.
-  destruct ds_d9aa as [ds_d9aa ds_d9aa_p].
-  induction ds_d9aa as [| n' IH_n'].
+  destruct ds_d9bO as [ds_d9bO ds_d9bO_p].
+  induction ds_d9bO as [| n' IH_n'].
   - refine (subsumptionCast
             Unit
             (λ (VV : Unit), ∃ (minus_res : MyNat_u), minus_rel O_u O_u minus_res ∧ minus_res == O_u)
@@ -79,15 +79,15 @@ Proof.
             ltac:(solver)).
 Qed.
 
-Definition add_0_r_spec (ds_d9ab : MyNat): Type :=
-  {{∃ (plus_res : MyNat_u), plus_rel ⌊ ds_d9ab -⌋ O_u plus_res ∧ plus_res == ⌊ ds_d9ab -⌋}}.
+Definition add_0_r_spec (ds_d9bP : MyNat): Type :=
+  {{∃ (plus_res : MyNat_u), plus_rel ⌊ ds_d9bP -⌋ O_u plus_res ∧ plus_res == ⌊ ds_d9bP -⌋}}.
 
 #[global] Hint Unfold add_0_r_spec: lia_unfold.
 
-Theorem add_0_r (ds_d9ab : MyNat): add_0_r_spec ds_d9ab.
+Theorem add_0_r (ds_d9bP : MyNat): add_0_r_spec ds_d9bP.
 Proof.
-  destruct ds_d9ab as [ds_d9ab ds_d9ab_p].
-  induction ds_d9ab as [| n' IH_n'].
+  destruct ds_d9bP as [ds_d9bP ds_d9bP_p].
+  induction ds_d9bP as [| n' IH_n'].
   - refine (subsumptionCast
             Unit
             (λ (VV : Unit), ∃ (plus_res : MyNat_u), plus_rel O_u O_u plus_res ∧ plus_res == O_u)
@@ -100,18 +100,18 @@ Proof.
             ltac:(solver)).
 Qed.
 
-Definition add_comm_spec (ds_d9ac m : MyNat): Type :=
+Definition add_comm_spec (ds_d9bQ m : MyNat): Type :=
   {{∃ (plus_res : MyNat_u),
-    plus_rel ⌊ ds_d9ac -⌋ ⌊ m -⌋ plus_res
-    ∧ ∃ (plus_res_2 : MyNat_u), plus_rel ⌊ m -⌋ ⌊ ds_d9ac -⌋ plus_res_2 ∧ plus_res == plus_res_2}}.
+    plus_rel ⌊ ds_d9bQ -⌋ ⌊ m -⌋ plus_res
+    ∧ ∃ (plus_res_2 : MyNat_u), plus_rel ⌊ m -⌋ ⌊ ds_d9bQ -⌋ plus_res_2 ∧ plus_res == plus_res_2}}.
 
 #[global] Hint Unfold add_comm_spec: lia_unfold.
 
-Theorem add_comm (ds_d9ac m : MyNat): add_comm_spec ds_d9ac m.
+Theorem add_comm (ds_d9bQ m : MyNat): add_comm_spec ds_d9bQ m.
 Proof.
-  destruct ds_d9ac as [ds_d9ac ds_d9ac_p].
+  destruct ds_d9bQ as [ds_d9bQ ds_d9bQ_p].
   destruct m as [m m_p].
-  destruct ds_d9ac as [| n'].
+  try revert m_p; generalize dependent m; induction ds_d9bQ as [| n' IH_n']; intros.
   - refine (subsumptionCast
             Unit
             (λ (VV : Unit),
@@ -121,9 +121,7 @@ Proof.
             (add_0_r (exist (λ (m : MyNat_u), MyNat_wf m ∧ True) m ltac:(solver)))
             ltac:(solver)).
   - assert (h_15156453 : plus n' m ==? plus m n').
-    { refine (add_comm
-              (exist (λ (VV : MyNat_u), MyNat_wf VV ∧ True) n' ltac:(solver))
-              (exist (λ (m : MyNat_u), MyNat_wf m ∧ True) m ltac:(solver))). }
+    { refine (IH_n' ltac:(try clear IH_n'; solver) m ltac:(try clear IH_n'; solver)). }
     refine (subsumptionCast
             Unit
             (λ (VV : Unit),
